@prefix aas: <https://admin-shell.io/aas/3/0/RC01/> .
@prefix iec61360: <https://admin-shell.io/DataSpecificationTemplates/DataSpecificationIEC61360/3/0/RC01/> .
@prefix phys_unit: <https://admin-shell.io/DataSpecificationTemplates/DataSpecificationPhysicalUnit/3/0/RC01/> .
@prefix dash: <http://datashapes.org/dash#> .
@prefix dc: <http://purl.org/dc/elements/1.1/> .
@prefix dcterms: <http://purl.org/dc/terms/> .
@prefix owl: <http://www.w3.org/2002/07/owl#> .
@prefix rdf: <http://www.w3.org/1999/02/22-rdf-syntax-ns#> .
@prefix rdfs: <http://www.w3.org/2000/01/rdf-schema#> .
@prefix vann: <http://purl.org/vocab/vann/> .
@prefix xsd: <http://www.w3.org/2001/XMLSchema#> .
@base <https://admin-shell.io/aas/3/0/RC01/> .

<https://admin-shell.io/aas/3/0/RC01/> rdf:type owl:Ontology ;
    vann:preferredNamespaceUri "https://admin-shell.io/aas/3/0/RC01/"^^xsd:anyURI ;
    owl:versionInfo "3.0.RC01" ;
    rdfs:comment "This ontology represents the data model for the Asset Administration Shell according to the specification 'Details of the Asset Administration Shell - Part 1 - Version 3.0.RC01'."@en ;
    vann:preferredNamespacePrefix "aas"^^xsd:string ;
    rdfs:isDefinedBy <https://admin-shell.io/aas/3/0/RC01/> ;
.

###  https://admin-shell.io/aas/3/0/RC01/AccessControl
aas:AccessControl rdf:type owl:Class ;
    rdfs:comment "Access Control defines the local access control policy administration point. Access Control has the major task to define the access permission rules."@en ;
    rdfs:label "Access Control"^^xsd:string ;
.

###  https://admin-shell.io/aas/3/0/RC01/AccessControl/accessPermissionRule
<https://admin-shell.io/aas/3/0/RC01/AccessControl/accessPermissionRule> rdf:type owl:ObjectProperty ;
    rdfs:comment "Access permission rules of the AAS describing the rights assigned to (already authenticated) subjects to access elements of the AAS."@en ;
    rdfs:label "has access permission rule"^^xsd:string ;
    rdfs:domain aas:AccessControl ;
    rdfs:range aas:AccessPermissionRule ;
.

###  https://admin-shell.io/aas/3/0/RC01/AccessControl/selectableSubjectAttributes
<https://admin-shell.io/aas/3/0/RC01/AccessControl/selectableSubjectAttributes> rdf:type owl:ObjectProperty ;
    rdfs:comment "Reference to a submodel defining the authenticated subjects that are configured for the AAS. They are selectable by the access permission rules to assign permissions to the subjects."@en ;
    rdfs:label "has selectable subject attributes"^^xsd:string ;
    rdfs:domain aas:AccessControl ;
    rdfs:range aas:Submodel ;
.

###  https://admin-shell.io/aas/3/0/RC01/AccessControl/defaultSubjectAttributes
<https://admin-shell.io/aas/3/0/RC01/AccessControl/defaultSubjectAttributes> rdf:type owl:ObjectProperty ;
    rdfs:comment "Reference to a submodel defining the default subjects attributes for the AAS that can be used to describe access permission rules."@en ;
    rdfs:label "has default subject attributes"^^xsd:string ;
    skos:note "The submodel is of kind=Type."@en ;
    rdfs:domain aas:AccessControl ;
    rdfs:range aas:Submodel ;
.

###  https://admin-shell.io/aas/3/0/RC01/AccessControl/selectablePermissions
<https://admin-shell.io/aas/3/0/RC01/AccessControl/selectablePermissions> rdf:type owl:ObjectProperty ;
    rdfs:comment "Reference to a submodel defining which permissions can be assigned to the subjects."@en ;
    rdfs:label "has selectable permissions"^^xsd:string ;
    skos:note "Default: reference to the submodel referenced via defaultPermissions"@en ;
    rdfs:domain aas:AccessControl ;
    rdfs:range aas:Submodel ;
.

###  https://admin-shell.io/aas/3/0/RC01/AccessControl/defaultPermissions
<https://admin-shell.io/aas/3/0/RC01/AccessControl/defaultPermissions> rdf:type owl:ObjectProperty ;
    rdfs:comment "Reference to a submodel defining the default permissions for the AAS."@en ;
    rdfs:label "has default permissions"^^xsd:string ;
    rdfs:domain aas:AccessControl ;
    rdfs:range aas:Submodel ;
.

###  https://admin-shell.io/aas/3/0/RC01/AccessControl/selectableEnvironmentAttributes
<https://admin-shell.io/aas/3/0/RC01/AccessControl/selectableEnvironmentAttributes> rdf:type owl:ObjectProperty ;
    rdfs:comment "Reference to a submodel defining which environment attributes can be accessed via the permission rules."@en ;
    rdfs:label "has selectable environment attributes"^^xsd:string ;
    rdfs:domain aas:AccessControl ;
    rdfs:range aas:Submodel ;
.

###  https://admin-shell.io/aas/3/0/RC01/AccessControl/defaultEnvironmentAttributes
<https://admin-shell.io/aas/3/0/RC01/AccessControl/defaultEnvironmentAttributes> rdf:type owl:ObjectProperty ;
    rdfs:comment "Reference to a submodel defining default environment attributes, i.e. attributes that are not describing the asset itself. The submodel is of kind=Type. At the same type the values of these environment attributes need to be accessible when evaluating the access permission rules. This is realized as a policy information point."@en ;
    rdfs:label "has default environment attributes"^^xsd:string ;
    rdfs:domain aas:AccessControl ;
    rdfs:range aas:Submodel ;
.

###  https://admin-shell.io/aas/3/0/RC01/AccessControlPolicyPoints
aas:AccessControlPolicyPoints rdf:type owl:Class ;
    rdfs:comment "Container for access control policy points."@en ;
    rdfs:label "Access ControlPolicy Points"^^xsd:string .

###  https://admin-shell.io/aas/3/0/RC01/AccessControlPolicyPoints/policyAdministrationPoint
<https://admin-shell.io/aas/3/0/RC01/AccessControlPolicyPoints/policyAdministrationPoint> rdf:type owl:ObjectProperty ;
    rdfs:comment "The access control administration policy point of the AAS."@en ;
    rdfs:label "has policy administration point"^^xsd:string ;
    rdfs:domain aas:AccessControlPolicyPoints ;
    rdfs:range aas:PolicyAdministrationPoint ;
.

###  https://admin-shell.io/aas/3/0/RC01/AccessControlPolicyPoints/policyDecisionPoint
<https://admin-shell.io/aas/3/0/RC01/AccessControlPolicyPoints/policyDecisionPoint> rdf:type owl:ObjectProperty ;
    rdfs:comment "The access control policy decision point of the AAS."@en ;
    rdfs:label "has policy decision point"^^xsd:string ;
    rdfs:domain aas:AccessControlPolicyPoints ;
    rdfs:range aas:PolicyDecisionPoint ;
.

###  https://admin-shell.io/aas/3/0/RC01/AccessControlPolicyPoints/policyEnforcementPoints
<https://admin-shell.io/aas/3/0/RC01/AccessControlPolicyPoints/policyEnforcementPoints> rdf:type owl:ObjectProperty ;
    rdfs:comment "The access control policy enforcement points of the AAS."@en ;
    rdfs:label "has policy enforcement points"^^xsd:string ;
    rdfs:domain aas:AccessControlPolicyPoints ;
    rdfs:range aas:PolicyEnforcementPoints ;
.

###  https://admin-shell.io/aas/3/0/RC01/AccessControlPolicyPoints/policyInformationPoints
<https://admin-shell.io/aas/3/0/RC01/AccessControlPolicyPoints/policyInformationPoints> rdf:type owl:ObjectProperty ;
    rdfs:comment "The access control policy information points of the AAS."@en ;
    rdfs:label "has policy information points"^^xsd:string ;
    rdfs:domain aas:AccessControlPolicyPoints ;
    rdfs:range aas:PolicyInformationPoints ;
.

###  https://admin-shell.io/aas/3/0/RC01/AccessPermissionRule
aas:AccessPermissionRule rdf:type owl:Class ;
    rdfs:subClassOf aas:Referable ;
    rdfs:subClassOf aas:Qualifiable ;
    rdfs:comment "Table that defines access permissions per authenticated subject for a set of objects (referable elements)."@en ;
    rdfs:label "Access Permission Rule"^^xsd:string ;
.

###  https://admin-shell.io/aas/3/0/RC01/AccessPermissionRule/permissionsPerObject
<https://admin-shell.io/aas/3/0/RC01/AccessPermissionRule/permissionsPerObject> rdf:type owl:ObjectProperty ;
    rdfs:comment "Set of object-permission pairs that define the permissions per object within the access permission rule."@en ;
    rdfs:label "has permissions per object"^^xsd:string ;
    rdfs:domain aas:AccessPermissionRule ;
    rdfs:range aas:PermissionsPerObject ;
.

###  https://admin-shell.io/aas/3/0/RC01/AccessPermissionRule/targetSubjectAttributes
<https://admin-shell.io/aas/3/0/RC01/AccessPermissionRule/targetSubjectAttributes> rdf:type owl:ObjectProperty ;
    rdfs:comment "Target subject attributes that need to be fulfilled by the accessing subject to get the permissions defined by this rule."@en ;
    rdfs:label "has target subject attributes"^^xsd:string ;
    rdfs:domain aas:AccessPermissionRule ;
    rdfs:range aas:SubjectAttributes ;
.

###  https://admin-shell.io/aas/3/0/RC01/AdministrativeInformation
aas:AdministrativeInformation rdf:type owl:Class ;
    rdfs:subClassOf aas:HasDataSpecification ;
    rdfs:comment "Every Identifiable may have administrative information. Administrative information includes for example 1) Information about the version of the element 2) Information about who created or who made the last change to the element 3) Information about the languages available in case the element contains text, for translating purposed also themmaster or default language may be definedIn the first version of the AAS metamodel only version information as defined by IEC 61360 is defined. In later versions additional attributes may be added."@en ;
    rdfs:label "Administrative Information"^^xsd:string ;
.

###  https://admin-shell.io/aas/3/0/RC01/AdministrativeInformation/version
<https://admin-shell.io/aas/3/0/RC01/AdministrativeInformation/version> rdf:type owl:DatatypeProperty ;
    rdfs:subPropertyOf dcterms:hasVersion ;
    rdfs:domain aas:AdministrativeInformation ;
    rdfs:range xsd:string ;
    rdfs:comment "Version of the element."@en ;
    rdfs:label "has version"^^xsd:string ;
.

###  https://admin-shell.io/aas/3/0/RC01/AdministrativeInformation/revision
<https://admin-shell.io/aas/3/0/RC01/AdministrativeInformation/revision> rdf:type owl:DatatypeProperty ;
    rdfs:subPropertyOf dcterms:hasVersion ;
    rdfs:comment "Revision of the element."@en ;
    skos:note "Constraint AASd-005: A revision requires a version. This means, if there is no version there is no revision neither."@en ;
    rdfs:label "has revision"^^xsd:string ;
    rdfs:domain aas:AdministrativeInformation ;
    rdfs:range xsd:string ;

.

###  https://admin-shell.io/aas/3/0/RC01/AnnotatedRelationshipElement
aas:AnnotatedRelationshipElement rdf:type owl:Class ;
    rdfs:subClassOf aas:RelationshipElement ;
    rdfs:comment "An annotated relationship element is an relationship element that can be annotated with additional data elements."@en ;
    rdfs:label "Annotated Relationship Element"^^xsd:string ;
.

###  https://admin-shell.io/aas/3/0/RC01/AnnotatedRelationshipElement/annotation
<https://admin-shell.io/aas/3/0/RC01/AnnotatedRelationshipElement/annotation> rdf:type owl:ObjectProperty ;
    rdfs:comment "Annotations that hold for the relationships between the two elements."@en ;
    rdfs:label "has annotation"^^xsd:string ;
    rdfs:domain aas:AnnotatedRelationshipElement ;
    rdfs:range aas:DataElement ;
.

###  https://admin-shell.io/aas/3/0/RC01/Asset
aas:Asset rdf:type owl:Class ;
    rdfs:subClassOf aas:HasDataSpecification , aas:Identifiable ;
    skos:altLabel "Object"@en ;
    skos:definition "Clearly identifiable asset for the Administration Shell"@en ;
    skos:prefLabel "Asset"@en ;
    rdfs:label "Asset"^^xsd:string ;
    skos:definition "Eindeutig identifizierbarer Gegenstand, der aufgrund seiner Bedeutung in der Informationswelt verwaltet wird"@de ;
    rdfs:comment "An Asset describes meta data of an asset that is represented by an AAS. The asset may either represent an asset type or an asset instance. The asset has a globally unique identifier plus - if needed - additional domain specific (proprietary) identifiers."@en ;
    skos:note "Objects may be known in the form of a type or of an instance. An object in the planning phase is known as a type"@en ;
.

###  https://admin-shell.io/aas/3/0/RC01/AssetInformation
aas:AssetInformation rdf:type owl:Class ;
    rdfs:comment "In AssetInformation identifying meta data of the asset that is represented by an AAS is defined."@en ;
    rdfs:comment "The asset may either represent an asset type or an asset instance."@en ;
	rdfs:comment "The asset has a globally unique identifier plus - if needed - additional domain specific (proprietary) identifiers. However, to support the corner case of very first phase of lifecycle where a stabilised/constant global asset identifier does not already exist, the corresponding attribute 'globalAssetId' is optional."@en ;
	rdfs:label "has Asset Identification Model"^^xsd:string ;
.

###  https://admin-shell.io/aas/3/0/RC01/AssetInformation/assetKind
<https://admin-shell.io/aas/3/0/RC01/AssetInformation/assetKind> rdf:type owl:ObjectProperty ;
    rdfs:domain aas:AssetInformation ;
    rdfs:range aas:AssetKind ;
    rdfs:label "has assetKind"^^xsd:string ;
    rdfs:comment "Denotes whether the Asset of of kind 'Type' or 'Instance'."@en ;
.

###  https://admin-shell.io/aas/3/0/RC01/AssetInformation/globalAssetId
<https://admin-shell.io/aas/3/0/RC01/AssetInformation/globalAssetId> rdf:type owl:ObjectProperty ;
    rdfs:domain aas:AssetInformation ;
    rdfs:range aas:Reference ;
    rdfs:comment "Reference to either an Asset object or a global reference to the asset the AAS is representing."@en ;
    rdfs:comment "This attribute is required as soon as the AAS is exchanged via partners in the life cycle of the asset. In a first phase of the life cycle the asset might not yet have a global id but already an internal identifier. The internal identifier would be modelled via 'externalAssetId'."@en ;
	rdfs:label "has global asset id"^^xsd:string ;
	skos:note "Constraint AASd-023: AssetInformation/globalAssetId either is a reference to an Asset object or a global reference."@en ;
.

###  https://admin-shell.io/aas/3/0/RC01/AssetInformation/externalAssetId
<https://admin-shell.io/aas/3/0/RC01/AssetInformation/externalAssetId> rdf:type owl:ObjectProperty ;
    rdfs:domain aas:AssetInformation ;
    rdfs:range aas:IdentifierKeyValuePair ;
    rdfs:comment "Additional domain specific external, typically proprietary Identifier for the asset like e.g. serial number etc."@en ;
	rdfs:label "has external asset id"^^xsd:string ;
.

###  https://admin-shell.io/aas/3/0/RC01/AssetInformation/billOfMaterial
<https://admin-shell.io/aas/3/0/RC01/AssetInformation/billOfMaterial> rdf:type owl:ObjectProperty ;
    rdfs:domain aas:AssetInformation ;
    rdfs:range aas:Submodel ;
    rdfs:comment "A reference to a Submodel that defines the bill of material of the asset represented by the AAS. This submodel contains a set of entities describing the material used to compose the composite I4.0 Component."@en ;
    rdfs:label "has Bill of Material"^^xsd:string ;
.

###  https://admin-shell.io/aas/3/0/RC01/AssetInformation/thumbnail
<https://admin-shell.io/aas/3/0/RC01/AssetInformation/thumbnail> rdf:type owl:ObjectProperty ;
    rdfs:domain aas:AssetInformation ;
    rdfs:range aas:File ;
    rdfs:label "has thumbnail"^^xsd:string ;
    rdfs:comment "Thumbnail of the asset represented by the asset administration shell."@en ;
.

###  https://admin-shell.io/aas/3/0/RC01/AssetAdministrationShell
aas:AssetAdministrationShell rdf:type owl:Class ;
    rdfs:subClassOf aas:HasDataSpecification , aas:Identifiable ;
    rdfs:label "Asset Administration Shell"^^xsd:string ;
    skos:altLabel "Administration Shell"@en , "Verwaltungsschale"@de ;
    skos:definition "Describes the Administration Shell for Assets, Products, Components, e.g. Machines"@en ;
    rdfs:comment "Describes the Administration Shell for Assets, Products, Components, e.g. Machines"@en ;
    skos:prefLabel "Asset Administration Shell"^^xsd:string ;
.

###  https://admin-shell.io/aas/3/0/RC01/AssetAdministrationShell/assetInformation
<https://admin-shell.io/aas/3/0/RC01/AssetAdministrationShell/assetInformation> rdf:type owl:ObjectProperty ;
    rdfs:domain aas:AssetAdministrationShell ;
    rdfs:range aas:AssetInformation ;
    rdfs:comment "Meta information about the asset the AAS is representing."@en ;
    rdfs:label "has assetInformation"^^xsd:string ;
.


###  https://admin-shell.io/aas/3/0/RC01/AssetAdministrationShell/derivedFrom
<https://admin-shell.io/aas/3/0/RC01/AssetAdministrationShell/derivedFrom> rdf:type owl:ObjectProperty ;
    rdfs:subPropertyOf <http://www.w3.org/TR/2013/REC-prov-o-20130430/#wasDerivedFrom> ;
    rdfs:domain aas:AssetAdministrationShell ;
    rdfs:range aas:Reference ;
    rdfs:comment "This relation connects instances of AAS with their respective types. Refer to Asset Kind for further information of instance and type kinds."@en ;
    rdfs:label "was derived from"^^xsd:string ;
.

###  https://admin-shell.io/aas/3/0/RC01/AssetAdministrationShell/security
<https://admin-shell.io/aas/3/0/RC01/AssetAdministrationShell/security> rdf:type owl:ObjectProperty ;
    rdfs:comment "Definition of the security relevant aspects of the AAS."@en ;
    rdfs:label "has security"^^xsd:string ;
    rdfs:domain aas:AssetAdministrationShell ;
    rdfs:range aas:Security ;
.

###  https://admin-shell.io/aas/3/0/RC01/AssetAdministrationShell/submodel
<https://admin-shell.io/aas/3/0/RC01/AssetAdministrationShell/submodel> rdf:type owl:ObjectProperty ;
    rdfs:domain aas:AssetAdministrationShell ;
    rdfs:range aas:Submodel ;
    rdfs:comment "Points from the Admin Shell to the Submodels that describe the Admin Shell of a given Asset"@en ;
    rdfs:label "has Submodel"^^xsd:string ;
.

###  https://admin-shell.io/aas/3/0/RC01/AssetAdministrationShell/view
<https://admin-shell.io/aas/3/0/RC01/AssetAdministrationShell/view> rdf:type owl:ObjectProperty ;
    rdfs:domain aas:AssetAdministrationShell;
    rdfs:range aas:View ;
    rdfs:comment "Points to the differents views associated to the Administration Shell via the Submodels."@en ;
    rdfs:label "has View"^^xsd:string ;
    skos:prefLabel "view"^^xsd:string ;
.

###  https://admin-shell.io/aas/3/0/RC01/AssetKind
aas:AssetKind rdf:type owl:Class ;
    rdfs:comment "Enumeration for denoting whether an element is a type or an instance."@en ;
    rdfs:label "Asset Kind"^^xsd:string  ;
    owl:oneOf (
        <https://admin-shell.io/aas/3/0/RC01/AssetKind/INSTANCE>
        <https://admin-shell.io/aas/3/0/RC01/AssetKind/TYPE>
    ) ;
.

###  https://admin-shell.io/aas/3/0/RC01/AssetKind/INSTANCE
<https://admin-shell.io/aas/3/0/RC01/AssetKind/INSTANCE> rdf:type aas:AssetKind ;
    rdfs:comment "Concrete, clearly identifiable component of a certain type."@en ;
    rdfs:label "Asset Instance"^^xsd:string ;
.

###  https://admin-shell.io/aas/3/0/RC01/AssetKind/TYPE
<https://admin-shell.io/aas/3/0/RC01/AssetKind/TYPE> rdf:type aas:AssetKind ;
    rdfs:comment "hardware or software element which specifies the common attributes shared by all instances of the type."@en ;
    rdfs:label "Asset Type"^^xsd:string ;
.

###  https://admin-shell.io/aas/3/0/RC01/BasicEvent
aas:BasicEvent rdf:type owl:Class ;
    rdfs:subClassOf aas:Event ;
    rdfs:label "Basic Event"^^xsd:string ;
    rdfs:comment "A basic event."@en ;
.

###  https://admin-shell.io/aas/3/0/RC01/BasicEvent/observed
<https://admin-shell.io/aas/3/0/RC01/BasicEvent/observed> rdf:type owl:ObjectProperty ;
    rdfs:comment "Reference to the data or other elements that are being observed."@en ;
    rdfs:label "observed by"^^xsd:string ;
    rdfs:domain aas:BasicEvent ;
    rdfs:range aas:Reference ;
.

###  https://admin-shell.io/aas/3/0/RC01/Blob
aas:Blob rdf:type owl:Class ;
    rdfs:subClassOf aas:DataElement ;
    rdfs:comment "A BLOB is a data element that represents a file that is contained with its source code in the value attribute."@en ;
    rdfs:label "Blob Data Element"^^xsd:string ;
	skos:note "Constraint AASd-057: The semanticId of a File or Blob submodel element shall only reference a ConceptDescription with the category DOCUMENT."@en ;
.

###  https://admin-shell.io/aas/3/0/RC01/Blob/mimeType
<https://admin-shell.io/aas/3/0/RC01/Blob/mimeType> rdf:type owl:DatatypeProperty ;
    rdfs:domain aas:Blob ;
    rdfs:range xsd:string ;
    rdfs:comment "Mime type of the content of the BLOB. The mime type states which file extension the file has. Valid values are e.g. 'application/json', 'application/xls', 'image/jpg' The allowed values are defined as in RFC2046."@en ;
    rdfs:label "has mimetype"^^xsd:string ;
    rdfs:seeAlso "http://uri4uri.net/vocab.html/#MimetypeDatatype"^^xsd:string ;
.

###  https://admin-shell.io/aas/3/0/RC01/Blob/value
<https://admin-shell.io/aas/3/0/RC01/Blob/value> rdf:type owl:ObjectProperty ;
    rdfs:domain aas:Blob ;
    rdfs:range xsd:byte ;
    rdfs:comment "The value of the BLOB instance of a blob data element."@en ;
    skos:note "In contrast to the file property the file content is stored directly as value in the Blob data element."@en ;
    rdfs:label "has value"^^xsd:string ;
.

###  https://admin-shell.io/aas/3/0/RC01/BlobCertificate
aas:BlobCertificate rdf:type owl:Class ;
    rdfs:subClassOf aas:Certificate ;
    rdfs:comment "Certificate provided as BLOB."@en ;
    rdfs:label "Blob Certificate"^^xsd:string ;
.

###  https://admin-shell.io/aas/3/0/RC01/BlobCertificate/blobCertificate
<https://admin-shell.io/aas/3/0/RC01/BlobCertificate/blobCertificate> rdf:type owl:DatatypeProperty ;
    rdfs:comment "Certificate as BLOB."@en ;
    rdfs:label "Blob Certificate"^^xsd:string ;
    rdfs:domain aas:BlobCertificate ;
    rdfs:range xsd:byte ;
.

###  https://admin-shell.io/aas/3/0/RC01/BlobCertificate/containedExtension
<https://admin-shell.io/aas/3/0/RC01/BlobCertificate/containedExtension> rdf:type owl:ObjectProperty ;
    rdfs:comment "Extensions contained in the certificate."@en ;
    rdfs:label "contains extension"^^xsd:string ;
    rdfs:domain aas:BlobCertificate ;
    rdfs:range aas:Reference ;
.

###  https://admin-shell.io/aas/3/0/RC01/BlobCertificate/lastCertificate
<https://admin-shell.io/aas/3/0/RC01/BlobCertificate/lastCertificate> rdf:type owl:DatatypeProperty ;
    rdfs:comment "Denotes whether this certificate is the certificated that fast added last."@en ;
    rdfs:label "is last certificate"^^xsd:string ;
    rdfs:domain aas:BlobCertificate ;
    rdfs:range xsd:boolean ;
.

###  https://admin-shell.io/aas/3/0/RC01/Capability
aas:Capability rdf:type owl:Class ;
    rdfs:subClassOf aas:SubmodelElement ;
    rdfs:comment "A capability is the implementation-independent description of the potential of an asset to achieve a certain effect in the physical or virtual world."@en ;
    rdfs:label "Capability"^^xsd:string ;
	skos:note "Constraint AASd-058: If the semanticId of a Capability submodel element references a ConceptDescription then the ConceptDescription/category shall be CAPABILITY."@en ;
.

###  https://admin-shell.io/aas/3/0/RC01/Category
aas:Category rdf:type owl:Class ;
    rdfs:comment "A enumeration for data elements except for files and blobs."@en ;
    rdfs:label "Category"^^xsd:string ;
    owl:oneOf (
        <https://admin-shell.io/aas/3/0/RC01/Category/PARAMETER>
        <https://admin-shell.io/aas/3/0/RC01/Category/VARIABLE>
        <https://admin-shell.io/aas/3/0/RC01/Category/CONSTANT>
    ) ;
.

###  https://admin-shell.io/aas/3/0/RC01/Category/CONSTANT
<https://admin-shell.io/aas/3/0/RC01/Category/CONSTANT> rdf:type aas:Category ;
    rdfs:comment "A constant property is a property with a value that does not change over time. In eCl@ss this kind of category has the category 'Coded Value'."@en ;
    rdfs:label "Constant"^^xsd:string ;
.

###  https://admin-shell.io/aas/3/0/RC01/Category/PARAMETER
<https://admin-shell.io/aas/3/0/RC01/Category/PARAMETER> rdf:type aas:Category ;
    rdfs:comment "A parameter property is a property that is once set and then typically does not change over time. This is for example the case for configuration parameters."@en ;
    rdfs:label "Parameter"^^xsd:string ;
.

###  https://admin-shell.io/aas/3/0/RC01/Category/VARIABLE
<https://admin-shell.io/aas/3/0/RC01/Category/VARIABLE> rdf:type aas:Category ;
    rdfs:comment "A variable property is a property that is calculated during runtime, i.e. its value is a runtime value."@en ;
    rdfs:label "Variable"^^xsd:string ;
.

###  https://admin-shell.io/aas/3/0/RC01/Certificate
aas:Certificate rdf:type owl:Class ;
    dash:abstract true ;
    rdfs:comment "A technical certificate proofing the identity through cryptographic measures."@en ;
    rdfs:label "Certificate"^^xsd:string ;
.

###  https://admin-shell.io/aas/3/0/RC01/Certificate/policyAdministrationPoint
<https://admin-shell.io/aas/3/0/RC01/Certificate/policyAdministrationPoint> rdf:type owl:ObjectProperty ;
    rdfs:comment "The access control administration policy point of the AAS."@en ;
    rdfs:label "has policy administration point"^^xsd:string ;
    rdfs:domain aas:Certificate ;
    rdfs:range aas:PolicyAdministrationPoint ;
.
###  https://admin-shell.io/aas/3/0/RC01/ConceptDescription
aas:ConceptDescription rdf:type owl:Class ;
    rdfs:subClassOf aas:HasDataSpecification , aas:Identifiable ;
    rdfs:label "Concept Description"^^xsd:string ;
    rdfs:comment "The semantics of a property or other elements that may have a semantic description is defined by a concept description. The description of the concept should follow a standardized schema (realized as data specification template)."@en ;
	skos:note "Constraint AASd-051: A ConceptDescription shall have one of the following categories: VALUE, PROPERTY, REFERENCE, DOCUMENT, CAPABILITY, RELATIONSHIP, COLLECTION, FUNCTION, EVENT, ENTITY, APPLICATION_CLASS, QUALIFIER, VIEW. Default: PROPERTY."@en ;
.

###  https://admin-shell.io/aas/3/0/RC01/ConceptDescription/content
<https://admin-shell.io/aas/3/0/RC01/ConceptDescription/content> rdf:type owl:ObjectProperty ;
    rdfs:subPropertyOf dcterms:identifier ;
    rdfs:comment "Link from a ConceptDescription to its explaining DataSpecificationContent."@en ;
    rdfs:label "has content"^^xsd:string ;
    rdfs:domain aas:ConceptDescription ;
    rdfs:range aas:DataSpecificationContent ;
.

###  https://admin-shell.io/aas/3/0/RC01/ConceptDescription/isCaseOf
<https://admin-shell.io/aas/3/0/RC01/ConceptDescription/isCaseOf> rdf:type owl:ObjectProperty ;
    rdfs:subPropertyOf dcterms:identifier ;
    rdfs:comment "Reference to an external definition the concept is compatible to or was derived from."@en ;
    skos:note "Compare to is-case-of relationship in ISO 13584-32 and IEC EN 61360."@en ;
    rdfs:label "is case of"^^xsd:string ;
    rdfs:domain aas:ConceptDescription ;
    rdfs:range aas:Reference ;
.

###  https://admin-shell.io/aas/3/0/RC01/Constraint
aas:Constraint rdf:type owl:Class ;
    dash:abstract true ;
    rdfs:comment "A constraint is used to further qualify an element."@en ;
    rdfs:label "Constraint"^^xsd:string ;
    skos:prefLabel "Constraint"@en ;
.

###  https://admin-shell.io/aas/3/0/RC01/DataElement
aas:DataElement rdf:type owl:Class ;
    rdfs:subClassOf aas:SubmodelElement ;
    dash:abstract true ;
    rdfs:comment "A data element is a submodel element that is not further composed out of other submodel elements. A data element is a submodel element that has a value. The type of value differs for different subtypes of data elements."@en ;
    rdfs:label "Data Element"^^xsd:string ;
.

###  https://admin-shell.io/aas/3/0/RC01/DataSpecificationContent
aas:DataSpecificationContent rdf:type owl:Class ;
    dash:abstract true ;
    rdfs:label "Data Specification Content"^^xsd:string ;
    rdfs:comment "DataSpecificationContent contains the additional attributes to be added to the element instance that references the data specification template and meta information about the template itself."@en ;
.

###  https://admin-shell.io/DataSpecificationTemplates/DataSpecificationIEC61360/3/0/RC01/DataSpecificationIEC61360
iec61360:DataSpecificationIEC61360 rdf:type owl:Class ;
    rdfs:subClassOf aas:DataSpecificationContent ;
    rdfs:label "Data Specification IEC 61360"^^xsd:string ;
    rdfs:comment "Data Specification Template for defining Property Descriptions conformant to IEC 61360."@en ;
	skos:note "Constraint AASd-075: For all ConceptDescriptions using data specification template IEC61360 (http://admin-shell.io/DataSpecificationTemplates/DataSpecificationIEC61360/2/0) values for the attributes not being marked as mandatory or optional in tables Table 9, Table 10, Table 11 and Table 12.depending on its category are ignored and handled as undefined."@en ;
.

###  https://admin-shell.io/DataSpecificationTemplates/DataSpecificationIEC61360/3/0/RC01/DataSpecificationIEC61360/dataType
<https://admin-shell.io/DataSpecificationTemplates/DataSpecificationIEC61360/3/0/RC01/DataSpecificationIEC61360/dataType> rdf:type owl:ObjectProperty ;
    rdfs:label "has datatype"^^xsd:string ;
    rdfs:domain iec61360:DataSpecificationIEC61360 ;
    rdfs:range iec61360:DataTypeIEC61360 ;
	skos:note "Constraint AASd-070: For a ConceptDescription with category PROPERTY or VALUE using data specification template IEC61360 (http://admin-shell.io/DataSpecificationTemplates/DataSpecificationIEC61360/2/0) -  DataSpecificationIEC61360/dataType is mandatory and shall be defined."@en ;
	skos:note "Constraint AASd-071: For a ConceptDescription with category REFERENCE using data specification template IEC61360 (http://admin-shell.io/DataSpecificationTemplates/DataSpecificationIEC61360/2/0) -  DataSpecificationIEC61360/dataType is STRING by default."@en ;
	skos:note "Constraint AASd-072: For a ConceptDescription with category DOCUMENT using data specification template IEC61360 (http://admin-shell.io/DataSpecificationTemplates/DataSpecificationIEC61360/2/0) -  DataSpecificationIEC61360/dataType shall be one of the following values: STRING or URL."@en ;
	skos:note "Constraint AASd-073: For a ConceptDescription with category QUALIFIER using data specification template IEC61360 (http://admin-shell.io/DataSpecificationTemplates/DataSpecificationIEC61360/2/0) -  DataSpecificationIEC61360/dataType is mandatory and shall be defined."@en ;
.

###  https://admin-shell.io/DataSpecificationTemplates/DataSpecificationIEC61360/3/0/RC01/DataSpecificationIEC61360/definition
<https://admin-shell.io/DataSpecificationTemplates/DataSpecificationIEC61360/3/0/RC01/DataSpecificationIEC61360/definition> rdf:type owl:ObjectProperty ;
    rdfs:label "has definition"^^xsd:string ;
    rdfs:domain iec61360:DataSpecificationIEC61360 ;
    rdfs:range rdf:langString ;
	skos:note "Constraint AASd-074: For all ConceptDescriptions except for ConceptDescriptions of category VALUE using data specification template IEC61360 (http://admin-shell.io/DataSpecificationTemplates/DataSpecificationIEC61360/2/0) -  DataSpecificationIEC61360/definition is mandatory and shall be defined at least in English."@en ;
.

###  https://admin-shell.io/DataSpecificationTemplates/DataSpecificationIEC61360/3/0/RC01/DataSpecificationIEC61360/levelType
<https://admin-shell.io/DataSpecificationTemplates/DataSpecificationIEC61360/3/0/RC01/DataSpecificationIEC61360/levelType> rdf:type owl:ObjectProperty ;
    rdfs:label "has level type"^^xsd:string ;
    rdfs:domain iec61360:DataSpecificationIEC61360 ;
    rdfs:range aas:LevelType ;
.

###  https://admin-shell.io/DataSpecificationTemplates/DataSpecificationIEC61360/3/0/RC01/DataSpecificationIEC61360/preferredName
<https://admin-shell.io/DataSpecificationTemplates/DataSpecificationIEC61360/3/0/RC01/DataSpecificationIEC61360/preferredName> rdf:type owl:DatatypeProperty ;
    rdfs:label "has preferred name"^^xsd:string ;
    rdfs:domain iec61360:DataSpecificationIEC61360 ;
    rdfs:range rdf:langString ;
.

###  https://admin-shell.io/DataSpecificationTemplates/DataSpecificationIEC61360/3/0/RC01/DataSpecificationIEC61360/shortName
<https://admin-shell.io/DataSpecificationTemplates/DataSpecificationIEC61360/3/0/RC01/DataSpecificationIEC61360/shortName> rdf:type owl:DatatypeProperty ;
    rdfs:label "has short name"^^xsd:string ;
    rdfs:domain iec61360:DataSpecificationIEC61360 ;
    rdfs:range rdf:langString ;
.

###  https://admin-shell.io/DataSpecificationTemplates/DataSpecificationIEC61360/3/0/RC01/DataSpecificationIEC61360/sourceOfDefinition
<https://admin-shell.io/DataSpecificationTemplates/DataSpecificationIEC61360/3/0/RC01/DataSpecificationIEC61360/sourceOfDefinition> rdf:type owl:DatatypeProperty ;
    rdfs:label "has source of definition"^^xsd:string ;
    rdfs:domain iec61360:DataSpecificationIEC61360 ;
    rdfs:range xsd:string ;
.

###  https://admin-shell.io/DataSpecificationTemplates/DataSpecificationIEC61360/3/0/RC01/DataSpecificationIEC61360/symbol
<https://admin-shell.io/DataSpecificationTemplates/DataSpecificationIEC61360/3/0/RC01/DataSpecificationIEC61360/symbol> rdf:type owl:DatatypeProperty ;
    rdfs:label "has symbol"^^xsd:string ;
    rdfs:domain iec61360:DataSpecificationIEC61360 ;
    rdfs:range xsd:string ;
.

###  https://admin-shell.io/DataSpecificationTemplates/DataSpecificationIEC61360/3/0/RC01/DataSpecificationIEC61360/unit
<https://admin-shell.io/DataSpecificationTemplates/DataSpecificationIEC61360/3/0/RC01/DataSpecificationIEC61360/unit> rdf:type owl:DatatypeProperty ;
    rdfs:label "has unit"^^xsd:string ;
    rdfs:domain iec61360:DataSpecificationIEC61360 ;
    rdfs:range xsd:string ;
.

###  https://admin-shell.io/DataSpecificationTemplates/DataSpecificationIEC61360/3/0/RC01/DataSpecificationIEC61360/unitId
<https://admin-shell.io/DataSpecificationTemplates/DataSpecificationIEC61360/3/0/RC01/DataSpecificationIEC61360/unitId> rdf:type owl:DatatypeProperty ;
    rdfs:label "has unit id"^^xsd:string ;
    rdfs:domain iec61360:DataSpecificationIEC61360 ;
    rdfs:range aas:Reference ;
.

###  https://admin-shell.io/DataSpecificationTemplates/DataSpecificationIEC61360/3/0/RC01/DataSpecificationIEC61360/valueFormat
<https://admin-shell.io/DataSpecificationTemplates/DataSpecificationIEC61360/3/0/RC01/DataSpecificationIEC61360/valueFormat> rdf:type owl:DatatypeProperty ;
    rdfs:label "has value format"^^xsd:string ;
    rdfs:domain iec61360:DataSpecificationIEC61360 ;
    rdfs:range xsd:string ;
.

###  https://admin-shell.io/DataSpecificationTemplates/DataSpecificationIEC61360/3/0/RC01/DataSpecificationIEC61360/value
<https://admin-shell.io/DataSpecificationTemplates/DataSpecificationIEC61360/3/0/RC01/DataSpecificationIEC61360/value> rdf:type owl:DatatypeProperty ;
    rdfs:label "has value"^^xsd:string ;
    rdfs:domain iec61360:DataSpecificationIEC61360 ;
    rdfs:range xsd:string ;
.

###  https://admin-shell.io/DataSpecificationTemplates/DataSpecificationIEC61360/3/0/RC01/DataSpecificationIEC61360/valueList
<https://admin-shell.io/DataSpecificationTemplates/DataSpecificationIEC61360/3/0/RC01/DataSpecificationIEC61360/valueList> rdf:type owl:DatatypeProperty ;
    rdfs:label "has value list"^^xsd:string ;
    rdfs:comment "The Type 'ValueList' lists all the allowed values for a concept description for which the allowed values are listed in an enumeration. The value list is a set of value reference pairs."@en ;
    rdfs:domain iec61360:DataSpecificationIEC61360 ;
    rdfs:range xsd:string ;
.

###  https://admin-shell.io/DataSpecificationTemplates/DataSpecificationIEC61360/3/0/RC01/DataSpecificationIEC61360/valueId
<https://admin-shell.io/DataSpecificationTemplates/DataSpecificationIEC61360/3/0/RC01/DataSpecificationIEC61360/valueId> rdf:type owl:ObjectProperty ;
    rdfs:label "has value id"^^xsd:string ;
    rdfs:domain iec61360:DataSpecificationIEC61360 ;
    rdfs:range aas:Reference ;
.

###  https://admin-shell.io/DataSpecificationTemplates/DataSpecificationPhysicalUnit/3/0/RC01/
phys_unit: rdf:type owl:Class ;
    rdfs:subClassOf aas:DataSpecificationContent ;
    rdfs:label "Data Specification Physical Unit"^^xsd:string ;
    rdfs:comment "Data Specification Template for Physical Units."@en ;
.

###  https://admin-shell.io/DataSpecificationTemplates/DataSpecificationPhysicalUnit/3/0/RC01/conversionFactor
phys_unit:conversionFactor rdf:type owl:DatatypeProperty ;
    rdfs:label "has conversion factor"^^xsd:string ;
    rdfs:domain phys_unit: ;
    rdfs:range xsd:string ;
.

###  https://admin-shell.io/DataSpecificationTemplates/DataSpecificationPhysicalUnit/3/0/RC01/definition
phys_unit:definition rdf:type owl:DatatypeProperty ;
    rdfs:label "has definition"^^xsd:string ;
    rdfs:domain phys_unit: ;
    rdfs:range rdf:langString ;
.

###  https://admin-shell.io/DataSpecificationTemplates/DataSpecificationPhysicalUnit/3/0/RC01/dinNotation
phys_unit:dinNotation rdf:type owl:DatatypeProperty ;
    rdfs:label "has DIN notation"^^xsd:string ;
    rdfs:domain phys_unit: ;
    rdfs:range xsd:string ;
.

###  https://admin-shell.io/DataSpecificationTemplates/DataSpecificationPhysicalUnit/3/0/RC01/eceCode
phys_unit:eceCode rdf:type owl:DatatypeProperty ;
    rdfs:label "has ECE code"^^xsd:string ;
    rdfs:domain phys_unit: ;
    rdfs:range xsd:string ;
.

###  https://admin-shell.io/DataSpecificationTemplates/DataSpecificationPhysicalUnit/3/0/RC01/eceName
phys_unit:eceName rdf:type owl:DatatypeProperty ;
    rdfs:label "has ECE name"^^xsd:string ;
    rdfs:domain phys_unit: ;
    rdfs:range xsd:string ;
.

###  https://admin-shell.io/DataSpecificationTemplates/DataSpecificationPhysicalUnit/3/0/RC01/nistName
phys_unit:nistName rdf:type owl:DatatypeProperty ;
    rdfs:label "has NIST name"^^xsd:string ;
    rdfs:domain phys_unit: ;
    rdfs:range xsd:string ;
.

###  https://admin-shell.io/DataSpecificationTemplates/DataSpecificationPhysicalUnit/3/0/RC01/siName
phys_unit:siName rdf:type owl:DatatypeProperty ;
    rdfs:label "has SI name"^^xsd:string ;
    rdfs:domain phys_unit: ;
    rdfs:range xsd:string ;
.

###  https://admin-shell.io/DataSpecificationTemplates/DataSpecificationPhysicalUnit/3/0/RC01/siNotation
phys_unit:siNotation rdf:type owl:DatatypeProperty ;
    rdfs:label "has SI notation"^^xsd:string ;
    rdfs:domain phys_unit: ;
    rdfs:range xsd:string ;
.

###  https://admin-shell.io/DataSpecificationTemplates/DataSpecificationPhysicalUnit/3/0/RC01/registrationAuthorityId
phys_unit:registrationAuthorityId rdf:type owl:DatatypeProperty ;
    rdfs:label "has registration authority"^^xsd:string ;
    rdfs:domain phys_unit: ;
    rdfs:range xsd:string ;
.

###  https://admin-shell.io/DataSpecificationTemplates/DataSpecificationPhysicalUnit/3/0/RC01/supplier
phys_unit:supplier rdf:type owl:DatatypeProperty ;
    rdfs:label "has supplier"^^xsd:string ;
    rdfs:domain phys_unit: ;
    rdfs:range xsd:string ;
.

###  https://admin-shell.io/DataSpecificationTemplates/DataSpecificationPhysicalUnit/3/0/RC01/unitName
phys_unit:unitName rdf:type owl:DatatypeProperty ;
    rdfs:label "unit has name"^^xsd:string ;
    rdfs:domain phys_unit: ;
    rdfs:range xsd:string ;
.

###  https://admin-shell.io/DataSpecificationTemplates/DataSpecificationPhysicalUnit/3/0/RC01/unitSymbol
phys_unit:unitSymbol rdf:type owl:DatatypeProperty ;
    rdfs:label "unit has symbol"^^xsd:string ;
    rdfs:domain phys_unit: ;
    rdfs:range xsd:string ;
.

###  https://admin-shell.io/aas/3/0/RC01/Entity
aas:Entity rdf:type owl:Class ;
    rdfs:subClassOf aas:SubmodelElement ;
    rdfs:label "Entity"^^xsd:string ;
    rdfs:comment "An entity is a submodel element that is used to model entities."@en ;
	skos:note "Constraint AASd-056: The semanticId of a Entity submodel element shall only reference a ConceptDescription with the category ENTITY. The ConceptDescription describes the elements assigned to the entity via Entity/statement."@en ;
.

###  https://admin-shell.io/aas/3/0/RC01/Entity/globalAssetId
<https://admin-shell.io/aas/3/0/RC01/Entity/globalAssetId> rdf:type owl:ObjectProperty ;
    rdfs:label "has global asset id"^^xsd:string ;
    rdfs:domain aas:Entity ;
    rdfs:range aas:Reference ;
    rdfs:comment "Reference to the asset the entity is representing."@en ;
    skos:note "The asset attribute must be set if entityType is set to 'SelfManagedEntity'. It is empty otherwise."@en ;
	skos:note "Constraint AASd-014: Either the attribute globalAssetId or externalAssetId of an Entity must be set if Entity/entityType is set to 'SelfManagedEntity'. They are not existing otherwise."@en ;
.

###  https://admin-shell.io/aas/3/0/RC01/Entity/externalAssetId
<https://admin-shell.io/aas/3/0/RC01/Entity/externalAssetId> rdf:type owl:ObjectProperty ;
    rdfs:label "has external asset id"^^xsd:string ;
    rdfs:domain aas:Entity ;
    rdfs:range aas:IdentifierKeyValuePair ;
    rdfs:comment "Reference to an identifier key value pair representing an external identifier of the asset represented by the asset administration shell. "@en ;
    skos:note "The asset attribute must be set if entityType is set to 'SelfManagedEntity'. It is empty otherwise."@en ;
    skos:note "Constraint AASd-014: Either the attribute globalAssetId or externalAssetId of an Entity must be set if Entity/entityType is set to 'SelfManagedEntity'. They are not existing otherwise."@en ;
.

###  https://admin-shell.io/aas/3/0/RC01/Entity/entityType
<https://admin-shell.io/aas/3/0/RC01/Entity/entityType> rdf:type owl:ObjectProperty ;
    rdfs:label "has entity type"^^xsd:string ;
    rdfs:domain aas:Entity ;
    rdfs:range aas:EntityType ;
    rdfs:comment "Describes whether the entity is a co-managed entity or a self-managed entity."@en ;
.

###  https://admin-shell.io/aas/3/0/RC01/Entity/statement
<https://admin-shell.io/aas/3/0/RC01/Entity/statement> rdf:type owl:DatatypeProperty ;
    rdfs:label "has statement"^^xsd:string ;
    rdfs:comment "Describes statements applicable to the entity by a set of submodel elements, typically with a qualified value."@en ;
    rdfs:domain aas:Entity ;
    rdfs:range aas:SubmodelElement ;
.

###  https://admin-shell.io/aas/3/0/RC01/EntityType
aas:EntityType rdf:type owl:Class ;
    rdfs:label "Entity Type"^^xsd:string ;
    rdfs:comment "Enumeration for denoting whether an entity is a self-managed entity or a co-managed entity."@en ;
    owl:oneOf (<https://admin-shell.io/aas/3/0/RC01/EntityType/CO_MANAGED_ENTITY> <https://admin-shell.io/aas/3/0/RC01/EntityType/SELF_MANAGED_ENTITY> ) ;
.

###  https://admin-shell.io/aas/3/0/RC01/EntityType/CO_MANAGED_ENTITY
<https://admin-shell.io/aas/3/0/RC01/EntityType/CO_MANAGED_ENTITY> rdf:type  aas:EntityType ;
    rdfs:comment "For co-managed entities there is no separate AAS. Co-managed entities need to be part of a self-managed entity."@en ;
    rdfs:label "Co-managed Entity"^^xsd:string ;
.

###  https://admin-shell.io/aas/3/0/RC01/EntityType/SELF_MANAGED_ENTITY
<https://admin-shell.io/aas/3/0/RC01/EntityType/SELF_MANAGED_ENTITY> rdf:type  aas:EntityType ;
    rdfs:comment "Self-Managed Entities have their own AAS but can be part of the bill of material of a composite self-managed entity. The asset of an I4.0 Component is a self-managed entity per definition."@en ;
    rdfs:label "Self-managed Entity"^^xsd:string ;
.

###  https://admin-shell.io/aas/3/0/RC01/Event
aas:Event rdf:type owl:Class ;
    rdfs:subClassOf aas:SubmodelElement ;
    dash:abstract true ;
    rdfs:label "Event"^^xsd:string ;
    rdfs:comment "An event."@en ;
	skos:note "Constraint AASd-061: The semanticId of a Event submodel element shall only reference a ConceptDescription with the category EVENT."@en ;
.

###  https://admin-shell.io/aas/3/0/RC01/EventElement
aas:EventElement rdf:type owl:Class ;
    rdfs:subClassOf aas:SubmodelElement ;
    rdfs:label "Event Element"^^xsd:string ;
    rdfs:comment "Defines the necessary information for sending or receiving events."@en ;
    skos:note "non-normative, just only for discussion (as of November 2019)."@en ;
.

###  https://admin-shell.io/aas/3/0/RC01/EventMessage
aas:EventMessage rdf:type owl:Class ;
    rdfs:subClassOf aas:SubmodelElement ;
    rdfs:label "Event Message"^^xsd:string ;
    rdfs:comment "Defines the necessary information of an event instance sent out or received."@en ;
    skos:note "non-normative, just only for discussion (as of November 2019)."@en ;
.

###  https://admin-shell.io/aas/3/0/RC01/File
aas:File rdf:type owl:Class ;
    rdfs:subClassOf aas:SubmodelElement ;
    rdfs:comment "A File is a data element that represents a file via its path description."@en ;
    rdfs:label "File Submodel Element"^^xsd:string ;
.

###  https://admin-shell.io/aas/3/0/RC01/File/mimeType
<https://admin-shell.io/aas/3/0/RC01/File/mimeType> rdf:type owl:DatatypeProperty ;
    rdfs:domain aas:File ;
    rdfs:range xsd:string ;
    rdfs:comment "Mime type of the content of the File."@en ;
    rdfs:label "has mimetype"^^xsd:string ;
    rdfs:seeAlso "http://uri4uri.net/vocab.html/#MimetypeDatatype"^^xsd:string ;
.

###  https://admin-shell.io/aas/3/0/RC01/File/value
<https://admin-shell.io/aas/3/0/RC01/File/value> rdf:type owl:ObjectProperty ;
    rdfs:domain aas:File ;
    rdfs:range xsd:string ;
    rdfs:comment "Path and name of the referenced file (with file extension). The path can be absolute or relative."@en ;
    rdfs:label "has value"^^xsd:string ;
.

###  https://admin-shell.io/aas/3/0/RC01/Formula
aas:Formula rdf:type owl:Class ;
    rdfs:subClassOf aas:Constraint ;
    dc:description "A formula is used to describe constraints by a logical expression."@en ;
    rdfs:label "Formula"^^xsd:string ;
.

###  https://admin-shell.io/aas/3/0/RC01/Formula/dependsOn
<https://admin-shell.io/aas/3/0/RC01/Formula/dependsOn> rdf:type owl:ObjectProperty ;
    rdfs:domain aas:Formula ;
    rdfs:range aas:Reference ;
    rdfs:comment "A formula may depend on referable or even external global elements - assumed that can be referenced and their value may be evaluated - that are used in the logical expression."@en ;
    rdfs:label "depends on"^^xsd:string ;
.
###  https://admin-shell.io/aas/3/0/RC01/HasDataSpecification
aas:HasDataSpecification rdf:type owl:Class ;
    dash:abstract true ;
    rdfs:comment "Element that can have be extended by using data specification templates. A data specification template defines the additional attributes an element may or shall have. The data specifications used are explicitly specified with their id."@en ;
    rdfs:label "Has Data Specification"^^xsd:string ;
	skos:note "Constraint AASd-050:  If the DataSpecificationContent DataSpecificationIEC61360 is used for an element then the value of hasDataSpecification/dataSpecification shall contain the global reference to the IRI of the corresponding data specification template https://admin-shell.io/DataSpecificationTemplates/DataSpecificationIEC61360/2/0."@en ;
.

###  https://admin-shell.io/aas/3/0/RC01/HasDataSpecification/dataSpecification
<https://admin-shell.io/aas/3/0/RC01/HasDataSpecification/dataSpecification> rdf:type owl:ObjectProperty ;
    rdfs:comment "Global reference to the data specification template used by the element."@en ;
    rdfs:label "has Data Specification"^^xsd:string ;
    rdfs:domain aas:HasDataSpecification ;
    rdfs:range aas:Reference ;
.

###  https://admin-shell.io/aas/3/0/RC01/HasKind
aas:HasKind rdf:type owl:Class ;
    dash:abstract true ;
    rdfs:comment "An element with a kind is an element that can either represent a type or an instance. Default for an element is that it is representing an instance."@en ;
    rdfs:label "Has Kind"^^xsd:string ;
.

###  https://admin-shell.io/aas/3/0/RC01/HasKind/kind
<https://admin-shell.io/aas/3/0/RC01/HasKind/kind> rdf:type owl:ObjectProperty ;
    rdfs:domain aas:HasKind ;
    rdfs:range aas:ModelingKind ;
    rdfs:label "has kind"^^xsd:string ;
    rdfs:comment "ModelingKind of the element: either type or instance."@en ;
.

###  https://admin-shell.io/aas/3/0/RC01/HasSemantics
aas:HasSemantics rdf:type owl:Class ;
    dash:abstract true ;
    rdfs:label "Has Semantics"^^xsd:string ;
    rdfs:comment "Element that can have a semantic definition. Identifier of the semantic definition of the element. It is called semantic id of the element. The semantic id may either reference an external global id or it may reference a referable model element of kind=Type that defines the semantics of the element."@en ;
    skos:note "In many cases the idShort is identical to the English short name within the semantic definition as referenced vi aits semantic id."@en ;
.

###  https://admin-shell.io/aas/3/0/RC01/HasSemantics/semanticId
<https://admin-shell.io/aas/3/0/RC01/HasSemantics/semanticId> rdf:type owl:ObjectProperty ;
    rdfs:subPropertyOf rdfs:seeAlso ;
    rdfs:label "has semantic ID"^^xsd:string ;
    skos:altLabel "has Semantic Expression"@en ;
    rdfs:comment "Points to the Expression Semantic of the Submodels"@en ;
    rdfs:comment "The semantic id might refer to an external information source, which explains the formulation of the submodel (for example an PDF if a standard)."@en ;
    rdfs:domain aas:HasSemantics ;
    rdfs:range aas:Reference ;
.

###  https://admin-shell.io/aas/3/0/RC01/Identifiable
aas:Identifiable rdf:type owl:Class ;
    dash:abstract true ;
    rdfs:subClassOf aas:Referable ;
    rdfs:comment "An element that has a globally unique identifier."@en ;
    rdfs:label "Identifiable"^^xsd:string ;
.

###  https://admin-shell.io/aas/3/0/RC01/Identifiable/administration
<https://admin-shell.io/aas/3/0/RC01/Identifiable/administration> rdf:type owl:ObjectProperty ;
    rdfs:comment "Administrative information of an identifiable element."@en ;
    skos:note "Some of the administrative information like the version number might need to be part of the identification."@en ;
    rdfs:label "has administration"^^xsd:string ;
    rdfs:domain aas:Identifiable ;
    rdfs:range aas:AdministrativeInformation ;
.

###  https://admin-shell.io/aas/3/0/RC01/Identifiable/identification
<https://admin-shell.io/aas/3/0/RC01/Identifiable/identification> rdf:type owl:ObjectProperty ;
    rdfs:domain aas:Identifiable ;
    rdfs:range aas:Identifier ;
    rdfs:label "has identification"^^xsd:string ;
    rdfs:comment "The globally unique identification of the element."@en ;
.

### https://admin-shell.io/aas/3/0/RC01/IdentifiableElements
aas:IdentifiableElements rdf:type owl:Class ;
    rdfs:subClassOf aas:ReferableElements ;
    rdfs:label "Identifiable Element"^^xsd:string ;
    rdfs:comment "Enumeration of all identifiable elements within an asset administration shell that are not identifiable"@en ;
    owl:oneOf (
        <https://admin-shell.io/aas/3/0/RC01/IdentifiableElements/ASSET>
        <https://admin-shell.io/aas/3/0/RC01/IdentifiableElements/ASSET_ADMINISTRATION_SHELL>
        <https://admin-shell.io/aas/3/0/RC01/IdentifiableElements/CONCEPT_DESCRIPTION>
        <https://admin-shell.io/aas/3/0/RC01/IdentifiableElements/SUBMODEL>
    ) ;
.

###  https://admin-shell.io/aas/3/0/RC01/IdentifiableElements/ASSET
<https://admin-shell.io/aas/3/0/RC01/IdentifiableElements/ASSET> rdf:type aas:IdentifiableElements ;
    rdfs:label "Asset"^^xsd:string ;
.

###  https://admin-shell.io/aas/3/0/RC01/IdentifiableElements/ASSET_ADMINISTRATION_SHELL
<https://admin-shell.io/aas/3/0/RC01/IdentifiableElements/ASSET_ADMINISTRATION_SHELL> rdf:type aas:IdentifiableElements ;
    rdfs:label "Asset Administration Shell"^^xsd:string ;
.

###  https://admin-shell.io/aas/3/0/RC01/IdentifiableElements/CONCEPT_DESCRIPTION_
<https://admin-shell.io/aas/3/0/RC01/IdentifiableElements/CONCEPT_DESCRIPTION> rdf:type aas:IdentifiableElements ;
    rdfs:label "Concept Description"^^xsd:string ;
.

###  https://admin-shell.io/aas/3/0/RC01/IdentifiableElements/SUBMODEL
<https://admin-shell.io/aas/3/0/RC01/IdentifiableElements/SUBMODEL> rdf:type aas:IdentifiableElements ;
    rdfs:label "Submodel"^^xsd:string ;
.

###  https://admin-shell.io/aas/3/0/RC01/Identifier
aas:Identifier rdf:type owl:Class ;
    rdfs:comment "Used to uniquely identify an entity by using an identifier."@en ;
    rdfs:label "Identifier"^^xsd:string ;
.

###  https://admin-shell.io/aas/3/0/RC01/Identifier/identifier
<https://admin-shell.io/aas/3/0/RC01/Identifier/identifier> rdf:type owl:DatatypeProperty ;
    rdfs:domain aas:Identifier ;
    rdfs:range rdfs:Literal ;
    rdfs:comment "A globally unique identifier which might not be a URI. Its type is defined in idType."@en ;
    rdfs:label "has identification"^^xsd:string ;
.

###  https://admin-shell.io/aas/3/0/RC01/Identifier/idType
<https://admin-shell.io/aas/3/0/RC01/Identifier/idType> rdf:type owl:ObjectProperty ;
    rdfs:comment "Type of the Identifier, e.g. IRI, IRDI etc. The supported Identifier types are defined in the enumeration 'IdentifierType'."@en ;
    rdfs:domain aas:Identifier ;
    rdfs:range aas:IdentifierType ;
    rdfs:label "has idType"^^xsd:string ;
.

### https://admin-shell.io/aas/3/0/RC01/IdentifierType
aas:IdentifierType rdf:type owl:Class ;
    rdfs:subClassOf aas:KeyType ;
    rdfs:label "Identifier Type"^^xsd:string ;
    rdfs:comment "Enumeration of different types of Identifiers for global identification"@en ;
    owl:oneOf (
        <https://admin-shell.io/aas/3/0/RC01/IdentifierType/IRDI>
        <https://admin-shell.io/aas/3/0/RC01/IdentifierType/IRI>
        <https://admin-shell.io/aas/3/0/RC01/IdentifierType/CUSTOM>
    ) ;
.

###  https://admin-shell.io/aas/3/0/RC01/IdentifierType/IRDI
<https://admin-shell.io/aas/3/0/RC01/IdentifierType/IRDI> rdf:type aas:IdentifierType ;
    rdfs:label "IRDI"^^xsd:string ;
    rdfs:comment "IRDI according to ISO29002-5 as an Identifier scheme for properties and classifications."@en ;
.

###  https://admin-shell.io/aas/3/0/RC01/IdentifierType/IRI
<https://admin-shell.io/aas/3/0/RC01/IdentifierType/IRI> rdf:type aas:IdentifierType ;
    rdfs:label "IRI"^^xsd:string ;
    rdfs:comment "IRI. Should only be used if unicode symbols are used that are not allowed in URI."@en ;
.

###  https://admin-shell.io/aas/3/0/RC01/IdentifierType/CUSTOM
<https://admin-shell.io/aas/3/0/RC01/IdentifierType/CUSTOM> rdf:type aas:IdentifierType ;
    rdfs:label "Custom"^^xsd:string ;
    rdfs:comment "Custom identifiers like GUIDs (globally unique Identifiers)"@en ;
.

###  https://admin-shell.io/aas/3/0/RC01/IdentifierKeyValuePair
aas:IdentifierKeyValuePair rdf:type owl:Class ;
    rdfs:subClassOf aas:HasSemantics ;
    rdfs:label "identifier key value pair"^^xsd:string ;
    rdfs:comment "An IdentifierKeyValuePair describes a generic identifier as key-value pair."@en ;
.

###  https://admin-shell.io/aas/3/0/RC01/IdentifierKeyValuePair/key
<https://admin-shell.io/aas/3/0/RC01/IdentifierKeyValuePair/key> rdf:type owl:DatatypeProperty ;
    rdfs:domain aas:IdentifierKeyValuePair ;
    rdfs:range xsd:string ;
    rdfs:comment "Key of the identifier."@en ;
    rdfs:label "has IdentifierKeyValuePair.key"^^xsd:string ;
.

###  https://admin-shell.io/aas/3/0/RC01/IdentifierKeyValuePair/value
<https://admin-shell.io/aas/3/0/RC01/IdentifierKeyValuePair/value> rdf:type owl:ObjectProperty ;
    rdfs:domain aas:IdentifierKeyValuePair ;
    rdfs:range xsd:string ;
    rdfs:comment "The value of the identifier with the corresponding key."@en ;
    rdfs:label "has IdentifierKeyValuePair.value"^^xsd:string ;
.

###  https://admin-shell.io/aas/3/0/RC01/IdentifierKeyValuePair/externalSubjectId
<https://admin-shell.io/aas/3/0/RC01/IdentifierKeyValuePair/externalSubjectId> rdf:type owl:ObjectProperty ;
    rdfs:domain aas:IdentifierKeyValuePair ;
    rdfs:range aas:Reference ;
    rdfs:comment "The (external) subject the key belongs to or has meaning to."@en ;
    rdfs:label "has IdentifierKeyValuePair.externalSubjectId"^^xsd:string ;
.

###  https://admin-shell.io/aas/3/0/RC01/Key
aas:Key rdf:type owl:Class ;
    rdfs:comment "A key is a reference to an element by its id."@en ;
    rdfs:label "Key"^^xsd:string ;
.

###  https://admin-shell.io/aas/3/0/RC01/Key/idType
<https://admin-shell.io/aas/3/0/RC01/Key/idType> rdf:type owl:ObjectProperty ;
    rdfs:comment "Type of the key value. In case of idType = idShort local shall be true. In case type=GlobalReference idType shall not be IdShort."@en ;
    rdfs:domain aas:Key ;
    rdfs:range aas:KeyType ;
    rdfs:label "has key type"^^xsd:string ;
	skos:note "Constraint AASd-080: In case Key/type == GlobalReference idType shall not be any LocalKeyType (IdShort, FragmentId)."@en ;
	skos:note "Constraint AASd-081: In case Key/type==AssetAdministrationShell Key/idType shall not be any  LocalKeyType (IdShort, FragmentId)."@en ;
.

###  https://admin-shell.io/aas/3/0/RC01/Key/type
<https://admin-shell.io/aas/3/0/RC01/Key/type> rdf:type owl:ObjectProperty ;
    rdfs:comment "Denote which kind of entity is referenced. In case type = GlobalReference then the element is a global unique id. In all other cases the key references a model element of the same or of another AAS. The name of the model element is explicitly listed."@en ;
    rdfs:label "has type"^^xsd:string ;
    rdfs:domain aas:Key ;
    rdfs:range aas:KeyElements ;
.

###  https://admin-shell.io/aas/3/0/RC01/Key/value
<https://admin-shell.io/aas/3/0/RC01/Key/value> rdf:type owl:DatatypeProperty ;
    rdfs:comment "The key value, for example an IRDI if the idType=IRDI."@en ;
    rdfs:label "has value"^^xsd:string ;
    rdfs:domain aas:Key ;
    rdfs:range xsd:string ;
.
###  https://admin-shell.io/aas/3/0/RC01/KeyElements
aas:KeyElements rdf:type owl:Class ;
    rdfs:label "Key Elements"^^xsd:string ;
    rdfs:comment "Enumeration of different key value types within a key. Contains KeyElements, ReferableElements, and IdentifiableElements."@en ;
    owl:oneOf (
        <https://admin-shell.io/aas/3/0/RC01/ReferableElements/ACCESS_PERMISSION_RULE>
        <https://admin-shell.io/aas/3/0/RC01/ReferableElements/ANNOTATED_RELATIONSHIP_ELEMENT>
        <https://admin-shell.io/aas/3/0/RC01/ReferableElements/BASIC_EVENT>
        <https://admin-shell.io/aas/3/0/RC01/ReferableElements/BLOB>
        <https://admin-shell.io/aas/3/0/RC01/ReferableElements/CAPABILITY>
        <https://admin-shell.io/aas/3/0/RC01/ReferableElements/CONCEPT_DICTIONARY>
        <https://admin-shell.io/aas/3/0/RC01/ReferableElements/GLOBAL_REFERENCE_KEY_ELEMENT>
        <https://admin-shell.io/aas/3/0/RC01/ReferableElements/DATA_ELEMENT>
        <https://admin-shell.io/aas/3/0/RC01/ReferableElements/FILE>
        <https://admin-shell.io/aas/3/0/RC01/ReferableElements/ENTITY>
        <https://admin-shell.io/aas/3/0/RC01/ReferableElements/EVENT>
        <https://admin-shell.io/aas/3/0/RC01/ReferableElements/MULTI_LANGUAGE_PROPERTY>
        <https://admin-shell.io/aas/3/0/RC01/ReferableElements/OPERATION>
        <https://admin-shell.io/aas/3/0/RC01/ReferableElements/PROPERTY>
        <https://admin-shell.io/aas/3/0/RC01/ReferableElements/RANGE>
        <https://admin-shell.io/aas/3/0/RC01/ReferableElements/REFERENCE_ELEMENT>
        <https://admin-shell.io/aas/3/0/RC01/ReferableElements/RELATIONSHIPT_ELEMENT>
        <https://admin-shell.io/aas/3/0/RC01/ReferableElements/SUBMODEL_ELEMENT>
        <https://admin-shell.io/aas/3/0/RC01/ReferableElements/SUBMODEL_ELEMENT_COLLECTION>
        <https://admin-shell.io/aas/3/0/RC01/ReferableElements/VIEW>

        <https://admin-shell.io/aas/3/0/RC01/IdentifableElements/ASSET>
        <https://admin-shell.io/aas/3/0/RC01/IdentifableElements/ASSET_ADMINISTRATION_SHELL>
        <https://admin-shell.io/aas/3/0/RC01/IdentifableElements/CONCEPT_DESCRIPTION>
        <https://admin-shell.io/aas/3/0/RC01/IdentifableElements/SUBMODEL>

        <https://admin-shell.io/aas/3/0/RC01/KeyElements/GLOBAL_REFERENCE>
        <https://admin-shell.io/aas/3/0/RC01/KeyElements/FRAGMENT_REFERENCE>
    ) ;
.

###  https://admin-shell.io/aas/3/0/RC01/KeyElements/GLOBAL_REFERENCE
<https://admin-shell.io/aas/3/0/RC01/KeyElements/GLOBAL_REFERENCE> rdf:type aas:KeyElements ;
    rdfs:label "Gobal Reference"^^xsd:string ;
    rdfs:comment "reference to an element not belonging to an asset administration shell"@en ;
.

###  https://admin-shell.io/aas/3/0/RC01/KeyElements/FRAGMENT_REFERENCE
<https://admin-shell.io/aas/3/0/RC01/KeyElements/FRAGMENT_REFERENCE> rdf:type aas:KeyElements ;
    rdfs:label "Fragement Reference"^^xsd:string ;
.

###  https://admin-shell.io/aas/3/0/RC01/KeyType
aas:KeyType rdf:type owl:Class ;
    rdfs:label "Key Type"^^xsd:string ;
    rdfs:comment "Enumeration of different key value types within a key. Contains IdentifierType and LocalKeyType."@en ;
    owl:oneOf (
        <https://admin-shell.io/aas/3/0/RC01/IdentifierType/IRDI>
        <https://admin-shell.io/aas/3/0/RC01/IdentifierType/IRI>
        <https://admin-shell.io/aas/3/0/RC01/IdentifierType/CUSTOM>

        <https://admin-shell.io/aas/3/0/RC01/LocalKeyType/IDSHORT>
        <https://admin-shell.io/aas/3/0/RC01/LocalKeyType/FRAGMENT_ID>
    ) ;
.

###  https://admin-shell.io/aas/3/0/RC01/LevelType
aas:LevelType rdf:type owl:Class ;
    rdfs:label "Level Type"^^xsd:string ;
    rdfs:comment "Enumeration of different level types within a DataSpecificationIEC61360. Contains Min, Max, Nom, and Typ."@en ;
    owl:oneOf (
        <https://admin-shell.io/aas/3/0/RC01/LevelType/MIN>
        <https://admin-shell.io/aas/3/0/RC01/LevelType/MAX>
        <https://admin-shell.io/aas/3/0/RC01/LevelType/NOM>
        <https://admin-shell.io/aas/3/0/RC01/LevelType/Typ>
    ) ;
.

###  https://admin-shell.io/aas/3/0/RC01/LevelType/MIN
<https://admin-shell.io/aas/3/0/RC01/LevelType/MIN> rdf:type aas:LevelType ;
    rdfs:label "MIN"^^xsd:string ;
    rdfs:comment "MIN according to IEC 61360 as an Identifier scheme for minimal levels."@en ;
.

###  https://admin-shell.io/aas/3/0/RC01/LevelType/MAX
<https://admin-shell.io/aas/3/0/RC01/LevelType/MAX> rdf:type aas:LevelType ;
    rdfs:label "MAX"^^xsd:string ;
    rdfs:comment "MAX according to IEC 61360 as an Identifier scheme for maximal levels."@en ;
.

###  https://admin-shell.io/aas/3/0/RC01/LevelType/NOM
<https://admin-shell.io/aas/3/0/RC01/LevelType/NOM> rdf:type aas:LevelType ;
    rdfs:label "NOM"^^xsd:string ;
    rdfs:comment "NOM according to IEC 61360 as an Identifier scheme for nominal levels."@en ;
.

###  https://admin-shell.io/aas/3/0/RC01/LevelType/TYP
<https://admin-shell.io/aas/3/0/RC01/LevelType/TYP> rdf:type aas:LevelType ;
    rdfs:label "TYP"^^xsd:string ;
    rdfs:comment "TYP according to IEC 61360 as an Identifier scheme for typical levels."@en ;
.

###  https://admin-shell.io/aas/3/0/RC01/LocalKeyType
aas:LocalKeyType rdf:type owl:Class ;
    rdfs:subClassOf aas:KeyType ;
    rdfs:label "Local Key Type"^^xsd:string ;
    rdfs:comment "Enumeration of different key value types within a key."@en ;
    owl:oneOf (
       <https://admin-shell.io/aas/3/0/RC01/LocalKeyType/IDSHORT>
       <https://admin-shell.io/aas/3/0/RC01/LocalKeyType/FRAGMENT_ID>
    ) ;
.

###  https://admin-shell.io/aas/3/0/RC01/LocalKeyType/IDSHORT
<https://admin-shell.io/aas/3/0/RC01/LocalKeyType/IDSHORT> rdf:type aas:LocalKeyType ;
    rdfs:label "IdShort"^^xsd:string ;
    rdfs:comment "idShort of a referable element"@en ;
.
###  https://admin-shell.io/aas/3/0/RC01/LocalKeyType/FRAGMENT_ID
<https://admin-shell.io/aas/3/0/RC01/LocalKeyType/FRAGMENT_ID> rdf:type aas:LocalKeyType ;
    rdfs:label "FragementId"^^xsd:string ;
    rdfs:comment "Identifier of a fragment within a file"@en ;
.

###  https://admin-shell.io/aas/3/0/RC01/ModelingKind
aas:ModelingKind rdf:type owl:Class ;
    rdfs:comment "Enumeration for denoting whether an element is a type or an instance."@en ;
    rdfs:label "Kind"^^xsd:string  ;
    owl:oneOf (
        aas:INSTANCE
        aas:TEMPLATE
    ) ;
.

###  https://admin-shell.io/aas/3/0/RC01/ModelingKind/INSTANCE
<https://admin-shell.io/aas/3/0/RC01/ModelingKind/INSTANCE> rdf:type  aas:ModelingKind ;
    rdfs:comment "Concrete, clearly identifiable component of a certain template."@en ;
    skos:note "It becomes an individual entity of a template, for example a device model, by defining specific property values."@en ;
    skos:note "In an object oriented view, an instance denotes an object (of a template) (class)."@en ;
    rdfs:label "Instance"^^xsd:string ;
.

###  https://admin-shell.io/aas/3/0/RC01/ModelingKind/TEMPLATE
<https://admin-shell.io/aas/3/0/RC01/ModelingKind/TEMPLATE> rdf:type  aas:ModelingKind ;
    rdfs:comment "Software element which specifies the common attributes shared by all instances of the template."@en ;
    rdfs:label "Template"^^xsd:string ;
.

###  https://admin-shell.io/aas/3/0/RC01/MultiLanguageProperty
aas:MultiLanguageProperty rdf:type owl:Class ;
    rdfs:subClassOf aas:DataElement ;
    rdfs:comment "A property is a data element that has a multi language value."@en ;
    rdfs:label "Multi Language Property"^^xsd:string ;
.

###  https://admin-shell.io/aas/3/0/RC01/MultiLanguageProperty/value
<https://admin-shell.io/aas/3/0/RC01/MultiLanguageProperty/value> rdf:type owl:ObjectProperty ;
    rdfs:comment "The value of the property instance."@en ;
    rdfs:label "has value"^^xsd:string ;
    rdfs:domain aas:MultiLanguageProperty ;
    rdfs:range rdf:langString ;
	skos:note "Constraint AASd-052b: If the semanticId of a MultiLanguageProperty references a ConceptDescription then the ConceptDescription/category shall be one of  following values: PROPERTY."@en ;
	skos:note "Constraint AASd-012: If both, the MultiLanguageProperty/value and the MultiLanguageProperty/valueId are present then for each string in a specific language the meaning must be the same as specified in MultiLanguageProperty/valueId."@en ;
	skos:note "Constraint AASd-067: If the semanticId of a MultiLanguageProperty references a ConceptDescription then DataSpecificationIEC61360/dataType shall be STRING_TRANSLATABLE."@en ;
.

###  https://admin-shell.io/aas/3/0/RC01/MultiLanguageProperty/valueId
<https://admin-shell.io/aas/3/0/RC01/MultiLanguageProperty/valueId> rdf:type owl:ObjectProperty ;
    rdfs:comment "Reference to the global unqiue id of a coded value."@en ;
    rdfs:label "hsa value Id"^^xsd:string ;
    rdfs:domain aas:MultiLanguageProperty ;
    rdfs:range aas:Reference ;
.

###  https://admin-shell.io/aas/3/0/RC01/ObjectAttributes
aas:ObjectAttributes rdf:type owl:Class ;
    rdfs:comment "A set of data elements that describe object attributes. These attributes need to refer to a data element within an existing submodel."@en ;
    rdfs:label "Object Attributes"^^xsd:string ;
.

###  https://admin-shell.io/aas/3/0/RC01/ObjectAttributes/objectAttribute
<https://admin-shell.io/aas/3/0/RC01/ObjectAttributes/objectAttribute> rdf:type owl:ObjectProperty ;
    rdfs:comment "A data elements that further classifies an object."@en ;
    rdfs:label "has object attribute"^^xsd:string ;
    rdfs:domain aas:ObjectAttributes ;
    rdfs:range aas:DataElement ;
.

###  https://admin-shell.io/aas/3/0/RC01/Operation
aas:Operation rdf:type owl:Class ;
    rdfs:subClassOf aas:SubmodelElement ;
    rdfs:comment "An operation is a submodel element with input and output variables."@en ;
    rdfs:label "Operation"^^xsd:string ;
	skos:note "Constraint AASd-060: The semanticId of a Operation submodel element shall only reference a ConceptDescription with the category FUNCTION."@en ;
.

###  https://admin-shell.io/aas/3/0/RC01/Operation/inputVariable
<https://admin-shell.io/aas/3/0/RC01/Operation/inputVariable> rdf:type owl:ObjectProperty ;
    rdfs:comment "Input parameter of the operation."@en ;
    rdfs:label "has input variable"^^xsd:string ;
    rdfs:domain aas:Operation ;
    rdfs:range aas:OperationVariable ;
.

###  https://admin-shell.io/aas/3/0/RC01/Operation/inoutputVariable
<https://admin-shell.io/aas/3/0/RC01/Operation/inoutputVariable> rdf:type owl:ObjectProperty ;
    rdfs:comment "Parameter that is input and output of the operation."@en ;
    rdfs:label "has input/output variable"^^xsd:string ;
    rdfs:domain aas:Operation ;
    rdfs:range aas:OperationVariable ;
.

###  https://admin-shell.io/aas/3/0/RC01/Operation/outputVariable
<https://admin-shell.io/aas/3/0/RC01/Operation/outputVariable> rdf:type owl:ObjectProperty ;
    rdfs:comment "Output parameter of the operation."@en ;
    rdfs:label "has output variable"^^xsd:string ;
    rdfs:domain aas:Operation ;
    rdfs:range aas:OperationVariable ;
.

###  https://admin-shell.io/aas/3/0/RC01/OperationVariable
aas:OperationVariable rdf:type owl:Class ;
    rdfs:comment "An operation variable is a submodel element that is used as input or output variable of an operation."@en ;
    rdfs:label "Operation Variable"^^xsd:string ;
.

###  https://admin-shell.io/aas/3/0/RC01/OperationVariable/value
<https://admin-shell.io/aas/3/0/RC01/OperationVariable/value> rdf:type owl:ObjectProperty ;
    rdfs:comment "Describes the needed argument for an operation via a submodel element of kind=Template."@en ;
    skos:note "The submodel element value of an operation variable shall be of kind=Template."@en ;
    rdfs:label "value"^^xsd:string ;
    rdfs:domain aas:OperationVariable ;
    rdfs:range aas:SubmodelElement ;
.

###  https://admin-shell.io/aas/3/0/RC01/Permission
aas:Permission rdf:type owl:Class ;
    rdfs:comment "Description of a single permission."@en ;
    rdfs:label "Permission"^^xsd:string ;
.

###  https://admin-shell.io/aas/3/0/RC01/Permission/kindOfPermission
<https://admin-shell.io/aas/3/0/RC01/Permission/kindOfPermission> rdf:type owl:ObjectProperty ;
    rdfs:comment "Description of the kind of permission. Possible kind of permission also include the denial of the permission."@en ;
    rdfs:label "has kind of permission"^^xsd:string ;
    rdfs:domain aas:Permission ;
    rdfs:range aas:PermissionKind ;
.

###  https://admin-shell.io/aas/3/0/RC01/Permission/permission
<https://admin-shell.io/aas/3/0/RC01/Permission/permission> rdf:type owl:ObjectProperty ;
    rdfs:comment "Reference to a property that defines the semantics of the permission."@en ;
    skos:note "Constraint AASs-010: The property referenced in Permission/permission shall have the category 'CONSTANT'."@en ;
    skos:note "Constraint AASs-011: The property referenced in Permission/permission shall be part of the submodel that is referenced within the 'selectablePermissions' attribute of 'AccessControl'."@en ;
    rdfs:label "has permission"^^xsd:string ;
    rdfs:domain aas:Permission ;
    rdfs:range aas:Property ;
.
###  https://admin-shell.io/aas/3/0/RC01/PermissionKind
aas:PermissionKind rdf:type owl:Class ;
    rdfs:comment "Enumeration of the kind of permissions that is given to the assignment of a permission to a subject."@en ;
    rdfs:label "Permission Kind"^^xsd:string ;
    owl:oneOf (
        <https://admin-shell.io/aas/3/0/RC01/PermissionKind/ALLOW>
        <https://admin-shell.io/aas/3/0/RC01/PermissionKind/DENY>
        <https://admin-shell.io/aas/3/0/RC01/PermissionKind/NOT_APPLICABLE>
        <https://admin-shell.io/aas/3/0/RC01/PermissionKind/UNDEFINED>
    ) ;
.

###  https://admin-shell.io/aas/3/0/RC01/PermissionKind/ALLOW
<https://admin-shell.io/aas/3/0/RC01/PermissionKind/ALLOW> rdf:type aas:PermissionKind ;
    rdfs:label "allow"^^xsd:string ;
    rdfs:comment "Allow the permission given to the subject."@en ;
.

###  https://admin-shell.io/aas/3/0/RC01/PermissionKind/DENY
<https://admin-shell.io/aas/3/0/RC01/PermissionKind/DENY> rdf:type aas:PermissionKind ;
    rdfs:label "deny"^^xsd:string ;
    rdfs:comment "Explicitly deny the permission given to the subject."@en ;
.

###  https://admin-shell.io/aas/3/0/RC01/PermissionKind/NOT_APPLICABLE
<https://admin-shell.io/aas/3/0/RC01/PermissionKind/NOT_APPLICABLE> rdf:type aas:PermissionKind ;
    rdfs:label "not applicable"^^xsd:string ;
    rdfs:comment "The permission is not applicable to the subject."@en ;
.

###  https://admin-shell.io/aas/3/0/RC01/PermissionKind/UNDEFINED
<https://admin-shell.io/aas/3/0/RC01/PermissionKind/UNDEFINED> rdf:type aas:PermissionKind ;
    rdfs:label "undefined"^^xsd:string ;
    rdfs:comment "It is undefined whether the permission is allowed, not applicable or denied to the subject."@en ;
.
###  https://admin-shell.io/aas/3/0/RC01/PermissionsPerObject
aas:PermissionsPerObject rdf:type owl:Class ;
    rdfs:comment "Table that defines access permissions for a specified object. The object is any referable element in the AAS. Additionally object attributes can be defined that further specify the kind of object the permissions apply to."@en ;
    rdfs:label "Permission Per Object"^^xsd:string ;
.

###  https://admin-shell.io/aas/3/0/RC01/PermissionsPerObject/object
<https://admin-shell.io/aas/3/0/RC01/PermissionsPerObject/object> rdf:type owl:ObjectProperty ;
    rdfs:comment "Element to which permission shall be assigned."@en ;
    rdfs:label "has object"^^xsd:string ;
    rdfs:domain aas:PermissionsPerObject ;
    rdfs:range aas:Referable ;
.

###  https://admin-shell.io/aas/3/0/RC01/PermissionsPerObject/permission
<https://admin-shell.io/aas/3/0/RC01/PermissionsPerObject/permission> rdf:type owl:ObjectProperty ;
    rdfs:comment "Permissions assigned to the object. The permissions hold for all subjects as specified in the access permission rule."@en ;
    rdfs:label "has object permission"^^xsd:string ;
    rdfs:domain aas:PermissionsPerObject ;
    rdfs:range aas:Permission ;
.

###  https://admin-shell.io/aas/3/0/RC01/PermissionsPerObject/targetObjectAttributes
<https://admin-shell.io/aas/3/0/RC01/PermissionsPerObject/targetObjectAttributes> rdf:type owl:ObjectProperty ;
    rdfs:comment "Target object attributes that need to be fulfilled so that the access permissions apply to the accessing subject."@en ;
    rdfs:label "has target object attributes"^^xsd:string ;
    rdfs:domain aas:PermissionsPerObject ;
    rdfs:range aas:ObjectAttributes ;
.

###  https://admin-shell.io/aas/3/0/RC01/PolicyAdministrationPoint
aas:PolicyAdministrationPoint rdf:type owl:Class ;
    rdfs:comment "Definition of a security administration point (PDP)."@en ;
    rdfs:label "Policy Administration Point"^^xsd:string ;
.

###  https://admin-shell.io/aas/3/0/RC01/PolicyAdministrationPoint/localAccessControl
<https://admin-shell.io/aas/3/0/RC01/PolicyAdministrationPoint/localAccessControl> rdf:type owl:ObjectProperty ;
    rdfs:comment "The policy administration point of access control as realized by the AAS itself."@en ;
    skos:note "Constraint AASd-009: Either there is an external policy administration point endpoint defined or the AAS has its own access control."@en ;
    rdfs:label "has local access control"^^xsd:string ;
    rdfs:domain aas:PolicyAdministrationPoint ;
    rdfs:range aas:AccessControl ;
.

###  https://admin-shell.io/aas/3/0/RC01/PolicyAdministrationPoint/externalAccessControl
<https://admin-shell.io/aas/3/0/RC01/PolicyAdministrationPoint/externalAccessControl> rdf:type owl:ObjectProperty ;
    rdfs:comment "Endpoint to an external access control defining a policy administration point to be used by the AAS."@en ;
    rdfs:label "has external access control"^^xsd:string ;
    rdfs:domain aas:PolicyAdministrationPoint ;
    rdfs:range xsd:boolean ;
.

###  https://admin-shell.io/aas/3/0/RC01/PolicyDecisionPoint
aas:PolicyDecisionPoint rdf:type owl:Class ;
    rdfs:comment "Defines a security policy decision point (PDP). "@en ;
    rdfs:label "Policy Decision Point"^^xsd:string ;
.

###  https://admin-shell.io/aas/3/0/RC01/PolicyDecisionPoint/externalPolicyDecisionPoints
<https://admin-shell.io/aas/3/0/RC01/PolicyDecisionPoint/externalPolicyDecisionPoints> rdf:type owl:DatatypeProperty ;
    rdfs:comment "If externalPolicyDecisionPoints True then Endpoints to external available decision points taking into consideration for access control for the AAS need to be configured."@en ;
    rdfs:label "is external policy decision point defined"^^xsd:string ;
    rdfs:domain aas:PolicyDecisionPoint ;
    rdfs:range xsd:boolean ;
.

###  https://admin-shell.io/aas/3/0/RC01/PolicyEnforcementPoints
aas:PolicyEnforcementPoints rdf:type owl:Class ;
    rdfs:comment "Defines the security policy enforcement points (PEP)."@en ;
    rdfs:label "Policy Enforcement Point"^^xsd:string ;
.

###  https://admin-shell.io/aas/3/0/RC01/PolicyEnforcementPoints/externalPolicyEnforcementPoint
<https://admin-shell.io/aas/3/0/RC01/PolicyEnforcementPoints/externalPolicyEnforcementPoint> rdf:type owl:DatatypeProperty ;
    rdfs:comment "If externalPolicyEnforcementPoint True then an Endpoint to external available enforcement point taking needs to be configured for the AAS."@en ;
    rdfs:label "is external policy enforcement point defined"^^xsd:string ;
    rdfs:domain aas:PolicyEnforcementPoints ;
    rdfs:range xsd:boolean ;
.

###  https://admin-shell.io/aas/3/0/RC01/PolicyInformationPoints
aas:PolicyInformationPoints rdf:type owl:Class ;
    rdfs:comment "Defines the security policy information points (PIP). Serves as the retrieval source of attributes, or the data required for policy evaluation to provide the information needed by the policy decision point to make the decisions."@en ;
    rdfs:label "Policy Information Points"^^xsd:string ;
.

###  https://admin-shell.io/aas/3/0/RC01/PolicyInformationPoints/externalInformationPoints
<https://admin-shell.io/aas/3/0/RC01/PolicyInformationPoints/externalInformationPoints> rdf:type owl:ObjectProperty ;
    rdfs:comment "If externalInformationPoints True then at least one Endpoint to external available information needs to be configured for the AAS."@en ;
    rdfs:label "has external information point"^^xsd:string ;
    rdfs:domain aas:PolicyInformationPoints ;
    rdfs:range xsd:boolean ;
.

###  https://admin-shell.io/aas/3/0/RC01/PolicyInformationPoints/internalInformationPoint
<https://admin-shell.io/aas/3/0/RC01/PolicyInformationPoints/internalInformationPoint> rdf:type owl:ObjectProperty ;
    rdfs:comment "References to submodels defining information used by security access permission rules."@en ;
    rdfs:label "has internal information point"^^xsd:string ;
    rdfs:domain aas:PolicyInformationPoints ;
    rdfs:range aas:Submodel ;
.

###  https://admin-shell.io/aas/3/0/RC01/Property
aas:Property rdf:type owl:Class ;
    rdfs:subClassOf aas:DataElement ;
    rdfs:comment "A property is a data element that has a single value."@en ;
    rdfs:label "Property"^^xsd:string ;
	skos:note "Constraint AASd-052a: If the semanticId of a Property references a ConceptDescription then the ConceptDescription/category shall be one of  following values: VALUE, PROPERTY."@en ;
	skos:note "Constraint AASd-065: If the semanticId of a Property or MultiLanguageProperty references a ConceptDescription with the  category VALUE then the value of the property is identical to  DataSpecificationIEC61360/value and the valueId of the property is identical to DataSpecificationIEC61360/valueId."@en ;
	skos:note "Constraint AASd-066: If the semanticId of a Property or MultiLanguageProperty references a ConceptDescription with the  category PROPERTY and DataSpecificationIEC61360/valueList is defined the value and valueId of the property is identical to one of the value reference pair types references in the value list, i.e. ValueReferencePairType/value or ValueReferencePairType/valueId, resp."@en ;
.

###  https://admin-shell.io/aas/3/0/RC01/Property/value
<https://admin-shell.io/aas/3/0/RC01/Property/value> rdf:type owl:ObjectProperty ;
    rdfs:comment "The value of the property instance."@en ;
    rdfs:label "has property value"^^xsd:string ;
    rdfs:domain aas:Property ;
    rdfs:range rdfs:Literal ;
.
###  https://admin-shell.io/aas/3/0/RC01/Property/valueId
<https://admin-shell.io/aas/3/0/RC01/Property/valueId> rdf:type owl:ObjectProperty ;
    rdfs:comment "Reference to the global unique id of a coded value."@en ;
    rdfs:label "has property value id"^^xsd:string ;
    skos:note "Constraint AASd-007: if both, the value and the valueId are present then the value needs to be identical to the value of the referenced coded value in valueId."@en ;
    rdfs:domain aas:Property ;
    rdfs:range aas:Reference ;
.

###  https://admin-shell.io/aas/3/0/RC01/Qualifiable
aas:Qualifiable rdf:type owl:Class ;
    dash:abstract true ;
    rdfs:comment "Additional qualification of a qualifiable element."@en ;
	skos:note "Constraint AASd-021: Every qualifiable can only have one qualifier with the same Qualifier/type."@en ;
    rdfs:label "Qualifiable"^^xsd:string ;
.

###  https://admin-shell.io/aas/3/0/RC01/Qualifiable/qualifier
<https://admin-shell.io/aas/3/0/RC01/Qualifiable/qualifier> rdf:type owl:ObjectProperty ;
    rdfs:comment "Additional qualification of a qualifiable element."@en ;
    rdfs:label "has qualifier"^^xsd:string ;
    rdfs:domain aas:Qualifiable ;
    rdfs:range aas:Constraint ;
.

###  https://admin-shell.io/aas/3/0/RC01/Qualifier
aas:Qualifier rdf:type owl:Class ;
    rdfs:subClassOf aas:Constraint ;
    rdfs:subClassOf aas:HasSemantics ;
    rdfs:comment "A qualifier is a type-value pair that makes additional statements w.r.t. the value of the element."@en ;
    rdfs:label "Qualifier"^^xsd:string ;
	skos:note "Constraint AASd-063: The semanticId of a Qualifier shall only reference a ConceptDescription with the category QUALIFIER."@en ;
.

###  https://admin-shell.io/aas/3/0/RC01/Qualifier/type
<https://admin-shell.io/aas/3/0/RC01/Qualifier/type> rdf:type owl:DatatypeProperty ;
    rdfs:comment "The qualifier type describes the type of the qualifier that is applied to the element."@en ;
    rdfs:label "has qualifier type"^^xsd:string ;
    rdfs:domain aas:Qualifier ;
    rdfs:range xsd:string ;
.

###  https://admin-shell.io/aas/3/0/RC01/Qualifier/value
<https://admin-shell.io/aas/3/0/RC01/Qualifier/value> rdf:type owl:ObjectProperty ;
    rdfs:comment "The qualifier value is the value of the qualifier."@en ;
    rdf:label "has qualifier value"^^xsd:string ;
    skos:note "Constraint AASd-006: if both, the value and the valueId are present then the value needs to be identical to the short name of the referenced coded value in qualifierValueId."@en ;
	skos:note "Constraint AASd-020: The value of Qualifier/value shall be consistent to the data type as defined in Qualifier/valueType."@en ;
    rdfs:domain aas:Qualifier ;
    rdfs:range rdfs:Literal ;
.

###  https://admin-shell.io/aas/3/0/RC01/Qualifier/valueId
<https://admin-shell.io/aas/3/0/RC01/Qualifier/valueId> rdf:type owl:ObjectProperty ;
    rdfs:comment "Reference to the global unqiue id of a coded value."@en ;
    rdf:label "has qualifier value id"^^xsd:string ;
    rdfs:domain aas:Qualifier ;
    rdfs:range aas:Reference ;
.

###  https://admin-shell.io/aas/3/0/RC01/Range
aas:Range rdf:type owl:Class ;
    rdfs:subClassOf aas:DataElement ;
    rdfs:comment "An element that is referable by its idShort. This id is not globally unique. This id is unique within the name space of the element."@en ;
    rdfs:label "Range"^^xsd:string ;
	skos:note "Constraint AASd-053: The semanticId of a Range submodel element shall only reference a ConceptDescription with the category PROPERTY."@en ;
	skos:note "Constraint AASd-068: If the semanticId of a  Range references a ConceptDescription then DataSpecificationIEC61360/dataType shall be a numerical one, i.e. REAL_* or RATIONAL_*."@en ;
	skos:note "Constraint AASd-069: If the semanticId of a  Range references a ConceptDescription then DataSpecificationIEC61360/levelType shall be identical to the set {Min,Max}."@en ;
.

###  https://admin-shell.io/aas/3/0/RC01/Range/max
<https://admin-shell.io/aas/3/0/RC01/Range/max> rdf:type owl:ObjectProperty ;
    rdfs:domain aas:Range ;
    rdfs:range rdfs:Literal ;
    rdfs:label "has maximum value"^^xsd:string ;
    rdfs:comment "The maximum value of the range."@en ;
.

###  https://admin-shell.io/aas/3/0/RC01/Range/min
<https://admin-shell.io/aas/3/0/RC01/Range/min> rdf:type owl:ObjectProperty ;
    rdfs:domain aas:Range ;
    rdfs:range rdfs:Literal ;
    rdfs:label "has minimum value"^^xsd:string ;
    rdfs:comment "The minimum value of the range."@en ;
.

###  https://admin-shell.io/aas/3/0/RC01/HasExtensions
aas:HasExtensions rdf:type owl:Class ;
    dash:abstract true ;
    rdfs:comment "Element that can be extended by proprietary extensions."@en ;
    rdfs:label "HasExtensions"^^xsd:string ;
.

###  https://admin-shell.io/aas/3/0/RC01/HasExtensions/extension
<https://admin-shell.io/aas/3/0/RC01/HasExtensions/extension> rdf:type owl:ObjectProperty ;
    rdfs:label "has extension"^^xsd:string ;
    rdfs:comment "An extension of the element."@en ;
    rdfs:domain aas:HasExtensions;
    rdfs:range aas:Extension;
.

###  https://admin-shell.io/aas/3/0/RC01/Extension
aas:Extension rdf:type owl:Class ;
    rdfs:subClassOf aas:HasSemantics ;
    rdfs:comment "Single extension of an element."@en ;
    rdfs:label "Extensions"^^xsd:string ;
	skos:note "Constraint AASd-077: The name of an extension within HasExtensions needs to be unique."@en ;
.

###  https://admin-shell.io/aas/3/0/RC01/Extension/name
<https://admin-shell.io/aas/3/0/RC01/Extension/name> rdf:type owl:DatatypeProperty ;
    rdfs:label "has extension name"^^xsd:string ;
    rdfs:comment "An extension of the element."@en ;
    rdfs:domain aas:Extension ;
    rdfs:range xsd:string ;
.

###  https://admin-shell.io/aas/3/0/RC01/Extension/valueType
<https://admin-shell.io/aas/3/0/RC01/Extension/valueType> rdf:type owl:DatatypeProperty ;
    rdfs:label "has extension value type"^^xsd:string ;
    rdfs:comment "Type of the value of the extension."@en ;
    rdfs:domain aas:Extension ;
    rdfs:range xsd:string ;
.

###  https://admin-shell.io/aas/3/0/RC01/Extension/value
<https://admin-shell.io/aas/3/0/RC01/Extension/value> rdf:type owl:ObjectProperty ;
    rdfs:label "has extension value"^^xsd:string ;
    rdfs:comment "Value of the extension."@en ;
    rdfs:domain aas:Extension ;
    rdfs:range xsd:string ;
.

###  https://admin-shell.io/aas/3/0/RC01/Extension/refersTo
<https://admin-shell.io/aas/3/0/RC01/Extension/refersTo> rdf:type owl:ObjectProperty ;
    rdfs:label "has extension reference to"^^xsd:string ;
    rdfs:comment "Reference to an element the extension refers to."@en ;
    rdfs:domain aas:Extension ;
    rdfs:range aas:Reference ;
.

###  https://admin-shell.io/aas/3/0/RC01/Referable
aas:Referable rdf:type owl:Class ;
    dash:abstract true ;
    rdfs:comment "An element that is referable by its idShort. This id is not globally unique. This id is unique within the name space of the element."@en ;
    rdfs:label "Referable"^^xsd:string ;
.

###  https://admin-shell.io/aas/3/0/RC01/Referable/referableCategory
<https://admin-shell.io/aas/3/0/RC01/Referable/referableCategory> rdf:type owl:DatatypeProperty ;
    rdfs:label "has category"^^xsd:string ;
    rdfs:comment "The category is a value that gives further meta information w.r.t. to the class of the element. It affects the expected existence of attributes and the applicability of constraints."@en ;
    rdfs:domain aas:Referable ;
    rdfs:range xsd:string ;
.

###  https://admin-shell.io/aas/3/0/RC01/Referable/description
<https://admin-shell.io/aas/3/0/RC01/Referable/description> rdf:type owl:DatatypeProperty ;
    rdfs:subPropertyOf rdfs:comment ;
    rdfs:label "has description"^^xsd:string ;
    rdfs:domain aas:Referable ;
    rdfs:range rdf:langString ;
    rdfs:comment "Description or comments on the element. The description can be provided in several languages."@en ;
.

###  https://admin-shell.io/aas/3/0/RC01/Referable/displayName
<https://admin-shell.io/aas/3/0/RC01/Referable/displayName> rdf:type owl:DatatypeProperty ;
    rdfs:subPropertyOf rdfs:comment ;
    rdfs:label "has display name"^^xsd:string ;
    rdfs:domain aas:Referable ;
    rdfs:range rdf:langString ;
    rdfs:comment "Display name. Can be provided in several languages."@en ;
.

###  https://admin-shell.io/aas/3/0/RC01/Referable/idShort
<https://admin-shell.io/aas/3/0/RC01/Referable/idShort> rdf:type owl:DatatypeProperty ;
    rdfs:subPropertyOf dcterms:identifier ;
    rdfs:label "has short id"^^xsd:string ;
    rdfs:comment "Identifying string of the element within its name space."@en ;
    skos:note "Constraint AASd-002: idShort shall only feature letters, digits, underscore ('_'); starting with a small letter. I.e. [a-z][a-zA-Z0-9_]+."@en ;
    skos:note "Constraint AASd-003: idShort shall be matched case-insensitive."@en ;
	skos:note "Constraint AASd-022: idShort of non-identifiable referables shall be unqiue in its namespace."@en ;
    skos:note "Note: In case the element is a property and the property has a semantic definition (HasSemantics) the idShort is typically identical to the short name in English. "@en ;
    skos:note "Note: In case of an identifiable element idShort is optional but recommended to be defined. It can be used for unique reference in its name space and thus allows better usability and a more performant implementation. In this case it is similar to the 'BrowserPath' in OPC UA."@en ;
    rdfs:domain aas:Referable ;
    rdfs:range xsd:string ;
.

###  https://admin-shell.io/aas/3/0/RC01/ReferableElements
aas:ReferableElements rdf:type owl:Class ;
    rdfs:subClassOf aas:KeyElements ;
    rdfs:label "Referable Elements"^^xsd:string ;
    rdfs:comment "Enumeration of all referable elements within an asset administration shell. Contains IdentifiableElements"@en ;
    owl:oneOf (
        <https://admin-shell.io/aas/3/0/RC01/ReferableElements/ACCESS_PERMISSION_RULE>
        <https://admin-shell.io/aas/3/0/RC01/ReferableElements/ANNOTATED_RELATIONSHIP_ELEMENT>
        <https://admin-shell.io/aas/3/0/RC01/ReferableElements/BASIC_EVENT>
        <https://admin-shell.io/aas/3/0/RC01/ReferableElements/BLOB>
        <https://admin-shell.io/aas/3/0/RC01/ReferableElements/CAPABILITY>
        <https://admin-shell.io/aas/3/0/RC01/ReferableElements/CONCEPT_DICTIONARY>
        <https://admin-shell.io/aas/3/0/RC01/ReferableElements/GLOBAL_REFERENCE_KEY_ELEMENT>
        <https://admin-shell.io/aas/3/0/RC01/ReferableElements/DATA_ELEMENT>
        <https://admin-shell.io/aas/3/0/RC01/ReferableElements/FILE>
        <https://admin-shell.io/aas/3/0/RC01/ReferableElements/ENTITY>
        <https://admin-shell.io/aas/3/0/RC01/ReferableElements/EVENT>
        <https://admin-shell.io/aas/3/0/RC01/ReferableElements/MULTI_LANGUAGE_PROPERTY>
        <https://admin-shell.io/aas/3/0/RC01/ReferableElements/OPERATION>
        <https://admin-shell.io/aas/3/0/RC01/ReferableElements/PROPERTY>
        <https://admin-shell.io/aas/3/0/RC01/ReferableElements/RANGE>
        <https://admin-shell.io/aas/3/0/RC01/ReferableElements/REFERENCE_ELEMENT>
        <https://admin-shell.io/aas/3/0/RC01/ReferableElements/RELATIONSHIPT_ELEMENT>
        <https://admin-shell.io/aas/3/0/RC01/ReferableElements/SUBMODEL_ELEMENT>
        <https://admin-shell.io/aas/3/0/RC01/ReferableElements/SUBMODEL_ELEMENT_COLLECTION>
        <https://admin-shell.io/aas/3/0/RC01/ReferableElements/VIEW>

        <https://admin-shell.io/aas/3/0/RC01/IdentifiableElements/ASSET>
        <https://admin-shell.io/aas/3/0/RC01/IdentifiableElements/ASSET_ADMINISTRATION_SHELL>
        <https://admin-shell.io/aas/3/0/RC01/IdentifiableElements/CONCEPT_DESCRIPTION>
        <https://admin-shell.io/aas/3/0/RC01/IdentifiableElements/SUBMODEL>
    ) ;
.

###  https://admin-shell.io/aas/3/0/RC01/ReferableElements/ACCESS_PERMISSION_RULE
<https://admin-shell.io/aas/3/0/RC01/ReferableElements/ACCESS_PERMISSION_RULE> rdf:type aas:ReferableElements ;
    rdfs:label "Access Permission Rule"^^xsd:string ;
.

###  https://admin-shell.io/aas/3/0/RC01/ReferableElements/ANNOTATED_RELATIONSHIP_ELEMENT
<https://admin-shell.io/aas/3/0/RC01/ReferableElements/ANNOTATED_RELATIONSHIP_ELEMENT> rdf:type aas:ReferableElements ;
    rdfs:label "Annotated relationship element"^^xsd:string ;
.

###  https://admin-shell.io/aas/3/0/RC01/ReferableElements/BASIC_EVENT
<https://admin-shell.io/aas/3/0/RC01/ReferableElements/BASIC_EVENT> rdf:type aas:ReferableElements ;
    rdfs:label "Basic Event"^^xsd:string ;
.
###  https://admin-shell.io/aas/3/0/RC01/ReferableElements/BLOB
<https://admin-shell.io/aas/3/0/RC01/ReferableElements/BLOB> rdf:type aas:ReferableElements ;
    rdfs:label "Blob"^^xsd:string ;
.

###  https://admin-shell.io/aas/3/0/RC01/ReferableElements/CAPABILITY
<https://admin-shell.io/aas/3/0/RC01/ReferableElements/CAPABILITY> rdf:type aas:ReferableElements ;
    rdfs:label "Capability"^^xsd:string ;
.

###  https://admin-shell.io/aas/3/0/RC01/ReferableElements/CONCEPT_DICTIONARY
<https://admin-shell.io/aas/3/0/RC01/ReferableElements/CONCEPT_DICTIONARY> rdf:type aas:ReferableElements ;
    rdfs:label "Concept Dictionary"^^xsd:string ;
.

###  https://admin-shell.io/aas/3/0/RC01/ReferableElements/DATA_ELEMENT
<https://admin-shell.io/aas/3/0/RC01/ReferableElements/DATA_ELEMENT> rdf:type aas:ReferableElements ;
    rdfs:label "Data Element"^^xsd:string ;
    skos:note "Data Element is abstract, i.e. if a key uses 'DataElement' the reference may be a Property, a File etc."@en ;
.

###  https://admin-shell.io/aas/3/0/RC01/ReferableElements/ENTITY
<https://admin-shell.io/aas/3/0/RC01/ReferableElements/ENTITY> rdf:type aas:ReferableElements ;
    rdfs:label "Entity"^^xsd:string ;
.

###  https://admin-shell.io/aas/3/0/RC01/ReferableElements/EVENT
<https://admin-shell.io/aas/3/0/RC01/ReferableElements/EVENT> rdf:type aas:ReferableElements ;
    rdfs:label "Event"^^xsd:string ;
    skos:note "Event is abstract"@en ;
.

###  https://admin-shell.io/aas/3/0/RC01/ReferableElements/MULTI_LANGUAGE_PROPERTY
<https://admin-shell.io/aas/3/0/RC01/ReferableElements/MULTI_LANGUAGE_PROPERTY> rdf:type aas:ReferableElements ;
    rdfs:label "Multi-language Property"^^xsd:string ;
    rdfs:comment "Property with a value that can be provided in multiple languages."@en ;
.

###  https://admin-shell.io/aas/3/0/RC01/ReferableElements/OPERATION
<https://admin-shell.io/aas/3/0/RC01/ReferableElements/OPERATION> rdf:type aas:ReferableElements ;
    rdfs:label "Operation"^^xsd:string ;
.
###  https://admin-shell.io/aas/3/0/RC01/ReferableElements/PROPERTY
<https://admin-shell.io/aas/3/0/RC01/ReferableElements/PROPERTY> rdf:type aas:ReferableElements ;
    rdfs:label "Property"^^xsd:string ;
.

###  https://admin-shell.io/aas/3/0/RC01/ReferableElements/RANGE
<https://admin-shell.io/aas/3/0/RC01/ReferableElements/RANGE> rdf:type aas:ReferableElements ;
    rdfs:label "Range"^^xsd:string ;
.

###  https://admin-shell.io/aas/3/0/RC01/ReferableElements/REFERENCE_ELEMENT
<https://admin-shell.io/aas/3/0/RC01/ReferableElements/REFERENCE_ELEMENT> rdf:type aas:ReferableElements ;
    rdfs:label "Reference Element"^^xsd:string ;
.

###  https://admin-shell.io/aas/3/0/RC01/ReferableElements/RELATIONSHIPT_ELEMENT
<https://admin-shell.io/aas/3/0/RC01/ReferableElements/RELATIONSHIPT_ELEMENT> rdf:type aas:ReferableElements ;
    rdfs:label "Relationship Element"^^xsd:string ;
.

###  https://admin-shell.io/aas/3/0/RC01/ReferableElements/SUBMODEL_ELEMENT
<https://admin-shell.io/aas/3/0/RC01/ReferableElements/SUBMODEL_ELEMENT> rdf:type aas:ReferableElements ;
    rdfs:label "Submodel Element"^^xsd:string ;
    skos:note "Submodel Element is abstract, i.e. if a key uses 'SubmodelElement' the reference may be a Property, a SubmodelElementCollection, an Operation etc."@en ;
.

###  https://admin-shell.io/aas/3/0/RC01/ReferableElements/SUBMODEL_ELEMENT_COLLECTION
<https://admin-shell.io/aas/3/0/RC01/ReferableElements/SUBMODEL_ELEMENT_COLLECTION> rdf:type aas:ReferableElements ;
    rdfs:label "Submodel Element Collection"^^xsd:string ;
    rdfs:comment "Collection of Submodel Elements"@en ;
.

###  https://admin-shell.io/aas/3/0/RC01/ReferableElements/VIEW
<https://admin-shell.io/aas/3/0/RC01/ReferableElements/VIEW> rdf:type aas:ReferableElements ;
    rdfs:label "View"^^xsd:string ;
.
###  https://admin-shell.io/aas/3/0/RC01/Reference
aas:Reference rdf:type owl:Class ;
    rdfs:comment "Reference to either a model element of the same or another AAs or to an external entity. A reference is an ordered list of keys, each key referencing an element. The complete list of keys may for example be concatenated to a path that then gives unique access to an element or entity."@en ;
    rdfs:label "Reference"^^xsd:string ;
.

###  https://admin-shell.io/aas/3/0/RC01/Reference/key
<https://admin-shell.io/aas/3/0/RC01/Reference/key> rdf:type owl:ObjectProperty ;
    rdfs:comment "Unique reference in its name space."@en ;
    rdfs:label "has key"^^xsd:string ;
    rdfs:domain aas:Reference ;
    rdfs:range aas:Key ;
.

###  https://admin-shell.io/aas/3/0/RC01/ReferenceElement
aas:ReferenceElement rdf:type owl:Class ;
    rdfs:subClassOf aas:DataElement ;
    rdfs:comment "A reference element is a data element that defines a logical reference to another element within the same or another AAS or a reference to an external object or entity."@en ;
    rdfs:label "Reference Element"^^xsd:string ;
	skos:note "Constraint AASd-054: The semanticId of a ReferenceElement shall only reference a ConceptDescription with the category REFERENCE."@en ;
.

###  https://admin-shell.io/aas/3/0/RC01/ReferenceElement/value
<https://admin-shell.io/aas/3/0/RC01/ReferenceElement/value> rdf:type owl:ObjectProperty ;
    rdfs:comment "Reference to any other referable element of the same of any other AAS or a reference to an external object or entity."@en ;
    rdfs:label "has reference value"^^xsd:string ;
    rdfs:domain aas:ReferenceElement ;
    rdfs:range aas:Reference ;
.

###  https://admin-shell.io/aas/3/0/RC01/RelationshipElement
aas:RelationshipElement rdf:type owl:Class ;
    rdfs:subClassOf aas:SubmodelElement ;
    dc:description "A relationship element is used to define a relationship between two referable elements."@en ;
    rdfs:label "Relationship Element"^^xsd:string ;
	skos:note "Constraint AASd-055: The semanticId of a RelationshipElement or a AnnotatedRelationshipElement shall only reference a ConceptDescription with the category RELATIONSHIP."@en ;
.

###  https://admin-shell.io/aas/3/0/RC01/RelationshipElement/first
<https://admin-shell.io/aas/3/0/RC01/RelationshipElement/first> rdf:type owl:ObjectProperty ;
    rdfs:comment "First element in the relationship taking the role of the subject."@en ;
    rdfs:label "has first relationship"^^xsd:string ;
    rdfs:domain aas:RelationshipElement ;
    rdfs:range aas:Referable ;
.

###  https://admin-shell.io/aas/3/0/RC01/RelationshipElement/second
<https://admin-shell.io/aas/3/0/RC01/RelationshipElement/second> rdf:type owl:ObjectProperty ;
    rdfs:comment "Second element in the relationship taking the role of the object."@en ;
    rdfs:label "has second relationship"^^xsd:string ;
    rdfs:domain aas:RelationshipElement ;
    rdfs:range aas:Referable ;
.

###  https://admin-shell.io/aas/3/0/RC01/Security
aas:Security rdf:type owl:Class ;
    rdfs:comment "Container for security relevant information of the AAS."@en ;
    rdfs:label "Security"^^xsd:string ;
.

###  https://admin-shell.io/aas/3/0/RC01/Security/accessControlPolicyPoints
<https://admin-shell.io/aas/3/0/RC01/Security/accessControlPolicyPoints> rdf:type owl:ObjectProperty ;
    rdfs:comment "Access control policy points of the AAS."@en ;
    rdfs:label "has access control policy points"^^xsd:string ;
    rdfs:domain aas:Security ;
    rdfs:range aas:PolicyAdministrationPoint ;
.

###  https://admin-shell.io/aas/3/0/RC01/Security/certificate
<https://admin-shell.io/aas/3/0/RC01/Security/certificate> rdf:type owl:ObjectProperty ;
    rdfs:comment "Certificates of the AAS."@en ;
    rdfs:label "has certificate"^^xsd:string ;
    rdfs:domain aas:Security ;
    rdfs:range aas:Certificate ;
.

###  https://admin-shell.io/aas/3/0/RC01/Security/requiredCertificateExtension
<https://admin-shell.io/aas/3/0/RC01/Security/requiredCertificateExtension> rdf:type owl:ObjectProperty ;
    rdfs:comment "Certificate extensions as required by the AAS."@en ;
    rdfs:label "has required certificate extension"^^xsd:string ;
    rdfs:domain aas:Security ;
    rdfs:range aas:Reference ;
.

###  https://admin-shell.io/aas/3/0/RC01/SubjectAttributes
aas:SubjectAttributes  rdf:type owl:Class ;
    rdfs:comment "A set of data elements that further classifies a specific subject."@en ;
    rdfs:label "Subject Attributes"^^xsd:string ;
.

###  https://admin-shell.io/aas/3/0/RC01/SubjectAttributes/subjectAttribute
<https://admin-shell.io/aas/3/0/RC01/SubjectAttributes/subjectAttribute> rdf:type owl:ObjectProperty ;
    rdfs:comment "A data element that further classifies a specific subject. "@en ;
    skos:note "Constraint AASs-015: The data element SubjectAttributes/subjectAttribute shall be part of the submodel that is referenced within the 'selectableSubjectAttributes' attribute of 'AccessControl'."@en ;
    rdfs:label "has subject attribute"^^xsd:string ;
    rdfs:domain aas:SubjectAttributes ;
    rdfs:range aas:DataElement ;
.

###  https://admin-shell.io/aas/3/0/RC01/Submodel
aas:Submodel rdf:type owl:Class ;
    rdfs:subClassOf aas:HasDataSpecification ;
    rdfs:subClassOf aas:HasKind ;
    rdfs:subClassOf aas:HasSemantics ;
    rdfs:subClassOf aas:Identifiable ;
    rdfs:subClassOf aas:Qualifiable ;
    rdfs:comment "A Submodel defines a specific aspect of the asset represented by the AAS. A submodel is used to structure the virtual representation and technical functionality of an Administration Shell into distinguishable parts. Each submodel refers to a well-defined domain or subject matter. Submodels can become standardized and thus become submodels types. Submodels can have different life-cycles."@en ,
    "Describe the different types of Data related to the I4.0 Asset"@en ;
    rdfs:label "Submodel"^^xsd:string ;
	skos:note "Constraint AASd-062: The semanticId of a Submodel shall only reference a ConceptDescription with the category APPLICATION_CLASS."@en ;
.

###  https://admin-shell.io/aas/3/0/RC01/Submodel/submodelElement
<https://admin-shell.io/aas/3/0/RC01/Submodel/submodelElement> rdf:type owl:ObjectProperty ;
    rdfs:domain aas:Submodel ;
    rdfs:range aas:SubmodelElement ;
    rdfs:comment "A submodel consists of zero or more submodel elements."@en ;
    rdfs:label "has Submodel Element"^^xsd:string ;
.

###  https://admin-shell.io/aas/3/0/RC01/SubmodelElement
aas:SubmodelElement rdf:type owl:Class ;
    rdfs:subClassOf aas:HasDataSpecification ;
    rdfs:subClassOf aas:HasKind ;
    rdfs:subClassOf aas:HasSemantics ;
    rdfs:subClassOf aas:Qualifiable ;
    rdfs:subClassOf aas:Referable ;
    dash:abstract true ;
    rdfs:comment "A submodel element is an element suitable for the description and differentiation of assets."@en ;
    rdfs:label "Submodel Element"^^xsd:string ;
    skos:note "The concept of type and instance applies to submodel elements. Properties are special submodel elements. The property types are defined in dictionaries (like the IEC Common Data Dictionary or eCl@ss), they do not have a value. The property type (kind=Type) is also called data element type in some standards. The property instances (kind=Instance) typically have a value. A property instance is also called property-value pair in certain standards."@en ;
.

###  https://admin-shell.io/aas/3/0/RC01/SubmodelElementCollection
aas:SubmodelElementCollection rdf:type owl:Class ;
    rdfs:subClassOf aas:SubmodelElement ;
    rdfs:comment "A submodel element collection is a set or list of submodel elements."@en ;
    rdfs:label "Submodel Element Collection"^^xsd:string ;
	skos:note "Constraint AASd-059: If the semanticId of a SubmodelElementCollection references a ConceptDescription then the category of the ConceptDescription shall be COLLECTION or ENTITY."@en ;
	skos:note "Constraint AASd-092: If the semanticId of a SubmodelElementCollection with SubmodelElementCollection/allowDuplicates == false references a ConceptDescription then the ConceptDescription/category shall be ENTITY."@en ;
	skos:note "Constraint AASd-093: If the semanticId of a SubmodelElementCollection with SubmodelElementCollection/allowDuplicates == true references a ConceptDescription then the ConceptDescription/category shall be COLLECTION."@en ;
.

###  https://admin-shell.io/aas/3/0/RC01/SubmodelElementCollection/allowDuplicates
<https://admin-shell.io/aas/3/0/RC01/SubmodelElementCollection/allowDuplicates> rdf:type owl:DatatypeProperty ;
    rdfs:comment "If allowDuplicates=true then it is allowed that the collection contains the same element several times. Default = false"@en ;
    rdfs:label "allow duplicates"^^xsd:string ;
    rdfs:domain aas:SubmodelElementCollection ;
    rdfs:range xsd:boolean ;
	skos:note "Constraint AASd-026: If allowDuplicates==false then it is not allowed that the collection contains several elements with the same semantics (i.e. the same semanticId)."@en ;
.

###  https://admin-shell.io/aas/3/0/RC01/SubmodelElementCollection/ordered
<https://admin-shell.io/aas/3/0/RC01/SubmodelElementCollection/ordered> rdf:type owl:DatatypeProperty ;
    rdfs:comment "If ordered=false then the elements in the property collection are not ordered. If ordered=true then the elements in the collection are ordered. Default = false"@en ;
    rdfs:label "ordered"^^xsd:string ;
    rdfs:domain aas:SubmodelElementCollection ;
    rdfs:range xsd:boolean ;
.

###  https://admin-shell.io/aas/3/0/RC01/SubmodelElementCollection/value
<https://admin-shell.io/aas/3/0/RC01/SubmodelElementCollection/value> rdf:type owl:ObjectProperty ;
    rdfs:comment "Submodel element contained in the collection."@en ;
    rdfs:label "has value"^^xsd:string ;
    rdfs:domain aas:SubmodelElementCollection ;
    rdfs:range aas:SubmodelElement ;
.

###  https://admin-shell.io/aas/3/0/RC01/View
aas:View rdf:type owl:Class ;
    rdfs:subClassOf aas:HasDataSpecification , aas:Referable , aas:HasSemantics ;
    rdfs:comment "A view is a collection of referable elements w.r.t. to a specific viewpoint of one or more stakeholders."@en ;
    rdfs:isDefinedBy "https://www.plattform-i40.de/I40/Redaktion/DE/Downloads/Publikation/hm-2018-trilaterale-coop.html"@de ;
    rdfs:label "View"^^xsd:string ;
	skos:note "Constraint AASd-064: If the semanticId of a View references a ConceptDescription then the category of the ConceptDescription shall be VIEW."@en ;
.

###  https://admin-shell.io/aas/3/0/RC01/View/containedElement
<https://admin-shell.io/aas/3/0/RC01/View/containedElement> rdf:type owl:ObjectProperty ;
    rdfs:comment "Referable elements that are contained in the view."@en ;
    rdfs:label "contains element"^^xsd:string ;
    rdfs:domain aas:View ;
    rdfs:range aas:Referable ;
.

### https://admin-shell.io/DataSpecificationTemplates/DataSpecificationIEC61360/3/0/RC01/DataTypeIEC61360
iec61360:DataTypeIEC61360 rdf:type owl:Class ;
    rdfs:label "Data Type IEC61360"^^xsd:string ;
    rdfs:comment "Enumeration of all IEC 61360 defined data types."@en ;
    owl:oneOf (
        iec61360:DATE
        iec61360:STRING
        iec61360:STRING_TRANSLATABLE
        iec61360:INTEGER_MEASURE
        iec61360:INTEGER_COUNT
        iec61360:INTEGER_CURRENCY
        iec61360:REAL_MEASURE
        iec61360:REAL_COUNT
        iec61360:REAL_CURRENCY
        iec61360:BOOLEAN
        iec61360:URL
        iec61360:RATIONAL
        iec61360:RATIONAL_MEASURE
        iec61360:TIME
        iec61360:TIMESTAMP
    ) ;
.

###  https://admin-shell.io/DataSpecificationTemplates/DataSpecificationIEC61360/3/0/RC01/DATE
iec61360:DATE rdf:type iec61360:DataTypeIEC61360 ;
    rdfs:label "date according to IEC61360"^^xsd:string ;
    rdfs:seeAlso xsd:date ;
.
###  https://admin-shell.io/DataSpecificationTemplates/DataSpecificationIEC61360/3/0/RC01/BOOLEAN
iec61360:BOOLEAN rdf:type iec61360:DataTypeIEC61360 ;
    rdfs:label "boolean according to IEC61360"^^xsd:string ;
    rdfs:seeAlso xsd:boolean ;
.
###  https://admin-shell.io/DataSpecificationTemplates/DataSpecificationIEC61360/3/0/RC01/INTEGER_CURRENCY
iec61360:INTEGER_CURRENCY rdf:type iec61360:DataTypeIEC61360 ;
    rdfs:label "integer currency according to IEC61360"^^xsd:string ;
.
###  https://admin-shell.io/DataSpecificationTemplates/DataSpecificationIEC61360/3/0/RC01/INTEGER_COUNT
iec61360:INTEGER_COUNT rdf:type iec61360:DataTypeIEC61360 ;
    rdfs:label "integer count according to IEC61360"^^xsd:string ;
.
###  https://admin-shell.io/DataSpecificationTemplates/DataSpecificationIEC61360/3/0/RC01/INTEGER_MEASURE
iec61360:INTEGER_MEASURE rdf:type iec61360:DataTypeIEC61360 ;
    rdfs:label "integer measure according to IEC61360"^^xsd:string ;
.
###  https://admin-shell.io/DataSpecificationTemplates/DataSpecificationIEC61360/3/0/RC01/INTEGER_CURRENCY
iec61360:INTEGER_CURRENCY rdf:type iec61360:DataTypeIEC61360 ;
    rdfs:label "real currency according to IEC61360"^^xsd:string ;
.
###  https://admin-shell.io/DataSpecificationTemplates/DataSpecificationIEC61360/3/0/RC01/REAL_COUNT
iec61360:REAL_COUNT rdf:type iec61360:DataTypeIEC61360 ;
    rdfs:label "real count according to IEC61360"^^xsd:string ;
.
###  https://admin-shell.io/DataSpecificationTemplates/DataSpecificationIEC61360/3/0/RC01/REAL_MEASURE
iec61360:REAL_MEASURE rdf:type iec61360:DataTypeIEC61360 ;
    rdfs:label "real measure according to IEC61360"^^xsd:string ;
.
###  https://admin-shell.io/DataSpecificationTemplates/DataSpecificationIEC61360/3/0/RC01/STRING
iec61360:STRING rdf:type iec61360:DataTypeIEC61360 ;
    rdfs:label "string according to IEC61360"^^xsd:string ;
    rdfs:seeAlso xsd:string ;
.
###  https://admin-shell.io/DataSpecificationTemplates/DataSpecificationIEC61360/3/0/RC01/STRING_TRANSLATABLE
iec61360:STRING_TRANSLATABLE rdf:type iec61360:DataTypeIEC61360 ;
    rdfs:label "translatable string according to IEC61360"^^xsd:string ;
    rdfs:seeAlso rdf:langString ;
.
###  https://admin-shell.io/DataSpecificationTemplates/DataSpecificationIEC61360/3/0/RC01/RATIONAL_MEASURE
iec61360:RATIONAL_MEASURE rdf:type iec61360:DataTypeIEC61360 ;
    rdfs:label "retional measure according to IEC61360"^^xsd:string ;
.
###  https://admin-shell.io/DataSpecificationTemplates/DataSpecificationIEC61360/3/0/RC01/RATIONAL
iec61360:RATIONAL rdf:type iec61360:DataTypeIEC61360 ;
    rdfs:label "retional according to IEC61360"^^xsd:string ;
.
###  https://admin-shell.io/DataSpecificationTemplates/DataSpecificationIEC61360/3/0/RC01/TIME
iec61360:TIME rdf:type iec61360:DataTypeIEC61360 ;
    rdfs:label "time according to IEC61360"^^xsd:string ;
.
###  https://admin-shell.io/DataSpecificationTemplates/DataSpecificationIEC61360/3/0/RC01/TIMESTAMP
iec61360:TIMESTAMP rdf:type iec61360:DataTypeIEC61360 ;
    rdfs:label "time stamp according to IEC61360"^^xsd:string ;
    rdfs:seeAlso xsd:dateTime ;
.
###  https://admin-shell.io/DataSpecificationTemplates/DataSpecificationIEC61360/3/0/RC01/URL
iec61360:URL rdf:type iec61360:DataTypeIEC61360 ;
    rdfs:label "url according to IEC61360"^^xsd:string ;
.
